<?xml version="1.0"?>
<rdf:RDF xmlns="http://www.semanticweb.org/delayed/cognitive-bias-ontology/InGroupBias#"
     xml:base="http://www.semanticweb.org/delayed/cognitive-bias-ontology/InGroupBias"
     xmlns:owl="http://www.w3.org/2002/07/owl#"
     xmlns:rdf="http://www.w3.org/1999/02/22-rdf-syntax-ns#"
     xmlns:xml="http://www.w3.org/XML/1998/namespace"
     xmlns:xsd="http://www.w3.org/2001/XMLSchema#"
     xmlns:rdfs="http://www.w3.org/2000/01/rdf-schema#"
     xmlns:terms="http://purl.org/dc/terms/"
     xmlns:InGroupBias="http://www.semanticweb.org/delayed/cognitive-bias-ontology/InGroupBias#"
     xmlns:InGroupBias1="https://raw.githubusercontent.com/Maedeam/KRKE-cognitive-biases/modeling-cognitive-biases/cognitive-biases/InGroupBias.owl#">
    <owl:Ontology rdf:about="https://raw.githubusercontent.com/Maedeam/KRKE-cognitive-biases/modeling-cognitive-biases/cognitive-biases/InGroupBias.owl">
        <terms:creator xml:lang="en">Atousa Heidarnia</terms:creator>
        <terms:creator xml:lang="en">Maede Hajjari</terms:creator>
        <terms:description xml:lang="en">In Group Bias module of the Cognitive Bias Ontology.</terms:description>
        <terms:hasVersion xml:lang="en">0.1</terms:hasVersion>
        <terms:title xml:lang="en">In Group Bias Ontology</terms:title>
        <rdfs:comment xml:lang="en">In-Group Bias, a prevalent cognitive bias, refers to the tendency of individuals to favor and show preferential treatment towards members of their own social, cultural, or identity group. This bias can lead to the perception of one&apos;s group as superior or more deserving than others, often resulting in a range of behaviors such as increased cooperation and empathy within the in-group and, conversely, discrimination or hostility towards out-groups. In-Group Bias is deeply rooted in social psychology, influencing how individuals perceive, interact with, and relate to those they consider part of their social circle.</rdfs:comment>
    </owl:Ontology>
    


    <!-- 
    ///////////////////////////////////////////////////////////////////////////////////////
    //
    // Annotation properties
    //
    ///////////////////////////////////////////////////////////////////////////////////////
     -->

    


    <!-- http://purl.org/dc/terms/creator -->

    <owl:AnnotationProperty rdf:about="http://purl.org/dc/terms/creator"/>
    


    <!-- http://purl.org/dc/terms/description -->

    <owl:AnnotationProperty rdf:about="http://purl.org/dc/terms/description"/>
    


    <!-- http://purl.org/dc/terms/hasVersion -->

    <owl:AnnotationProperty rdf:about="http://purl.org/dc/terms/hasVersion"/>
    


    <!-- http://purl.org/dc/terms/title -->

    <owl:AnnotationProperty rdf:about="http://purl.org/dc/terms/title"/>
    


    <!-- 
    ///////////////////////////////////////////////////////////////////////////////////////
    //
    // Object Properties
    //
    ///////////////////////////////////////////////////////////////////////////////////////
     -->

    


    <!-- https://raw.githubusercontent.com/Maedeam/KRKE-cognitive-biases/modeling-cognitive-biases/cognitive-biases/InGroupBias.owl#causedBy -->

    <owl:ObjectProperty rdf:about="https://raw.githubusercontent.com/Maedeam/KRKE-cognitive-biases/modeling-cognitive-biases/cognitive-biases/InGroupBias.owl#causedBy">
        <rdfs:domain rdf:resource="https://raw.githubusercontent.com/Maedeam/KRKE-cognitive-biases/modeling-cognitive-biases/cognitive-biases/InGroupBias.owl#Loyality"/>
        <rdfs:domain rdf:resource="https://w3id.org/framester/data/framestercore/Competition"/>
        <rdfs:domain rdf:resource="https://w3id.org/framester/data/framestercore/Supporting"/>
        <rdfs:range rdf:resource="https://w3id.org/framester/data/framestercore/Categorization"/>
        <rdfs:label xml:lang="en">causedBy</rdfs:label>
    </owl:ObjectProperty>
    


    <!-- https://w3id.org/affectedBy -->

    <owl:ObjectProperty rdf:about="https://w3id.org/affectedBy">
        <rdfs:domain rdf:resource="http://www.ontologydesignpatterns.org/cp/owl/agentrole.owl#Agent"/>
        <rdfs:domain rdf:resource="http://www.ontologydesignpatterns.org/cp/owl/agentrole.owl#GroupMember"/>
        <rdfs:range rdf:resource="https://w3id.org/framester/data/framestercore/Categorization"/>
        <rdfs:comment xml:lang="en">A relation between qualities or entities.</rdfs:comment>
        <rdfs:label xml:lang="en">affectedBy</rdfs:label>
    </owl:ObjectProperty>
    


    <!-- https://w3id.org/affectedBy#belongsTo -->

    <owl:ObjectProperty rdf:about="https://w3id.org/affectedBy#belongsTo">
        <rdfs:domain rdf:resource="http://www.ontologydesignpatterns.org/cp/owl/agentrole.owl#Agent"/>
        <rdfs:domain rdf:resource="http://www.ontologydesignpatterns.org/cp/owl/agentrole.owl#GroupMember"/>
        <rdfs:range rdf:resource="https://w3id.org/framester/data/framestercore/Organization#SocialGroup"/>
        <rdfs:comment xml:lang="en">A relation between qualities and features of interest.</rdfs:comment>
        <rdfs:label xml:lang="en">belongsTo</rdfs:label>
    </owl:ObjectProperty>
    


    <!-- https://w3id.org/affectedBy#influencedBy -->

    <owl:ObjectProperty rdf:about="https://w3id.org/affectedBy#influencedBy">
        <rdfs:domain rdf:resource="http://www.ontologydesignpatterns.org/cp/owl/agentrole.owl#Agent"/>
        <rdfs:domain rdf:resource="http://www.ontologydesignpatterns.org/cp/owl/agentrole.owl#GroupMember"/>
        <rdfs:range rdf:resource="https://w3id.org/framester/data/framestercore/Categorization"/>
        <rdfs:comment xml:lang="en">When an agent&apos;s decision is influenced by an external entity.</rdfs:comment>
        <rdfs:label xml:lang="en">influencedBy</rdfs:label>
    </owl:ObjectProperty>
    


    <!-- 
    ///////////////////////////////////////////////////////////////////////////////////////
    //
    // Classes
    //
    ///////////////////////////////////////////////////////////////////////////////////////
     -->

    


    <!-- http://www.ontologydesignpatterns.org/cp/owl/agentrole.owl#Agent -->

    <owl:Class rdf:about="http://www.ontologydesignpatterns.org/cp/owl/agentrole.owl#Agent">
        <owl:equivalentClass rdf:resource="http://www.ontologydesignpatterns.org/cp/owl/agentrole.owl#GroupMember"/>
        <rdfs:comment xml:lang="en">Any physical or social agent, including a person, a social group, or an organization.</rdfs:comment>
        <rdfs:label xml:lang="en">Agent</rdfs:label>
    </owl:Class>
    


    <!-- http://www.ontologydesignpatterns.org/cp/owl/agentrole.owl#GroupMember -->

    <owl:Class rdf:about="http://www.ontologydesignpatterns.org/cp/owl/agentrole.owl#GroupMember">
        <rdfs:comment xml:lang="en">Represents an individual belonging to a social group.</rdfs:comment>
        <rdfs:label xml:lang="en">GroupMember</rdfs:label>
    </owl:Class>
    


    <!-- https://raw.githubusercontent.com/Maedeam/KRKE-cognitive-biases/modeling-cognitive-biases/cognitive-biases/InGroupBias.owl#Loyality -->

    <owl:Class rdf:about="https://raw.githubusercontent.com/Maedeam/KRKE-cognitive-biases/modeling-cognitive-biases/cognitive-biases/InGroupBias.owl#Loyality">
        <owl:equivalentClass rdf:resource="https://w3id.org/framester/data/framestercore/Supporting"/>
        <rdfs:comment xml:lang="en">Loyalty is a steadfast and faithful commitment or allegiance to a person, group, cause, or organization.</rdfs:comment>
        <rdfs:label xml:lang="en">Loyality</rdfs:label>
    </owl:Class>
    


    <!-- https://w3id.org/framester/data/framestercore/Categorization -->

    <owl:Class rdf:about="https://w3id.org/framester/data/framestercore/Categorization">
        <rdfs:comment xml:lang="en">Represents the process of classifying individuals based on certain criteria.</rdfs:comment>
        <rdfs:label xml:lang="en">Categorization</rdfs:label>
    </owl:Class>
    


    <!-- https://w3id.org/framester/data/framestercore/Competition -->

    <owl:Class rdf:about="https://w3id.org/framester/data/framestercore/Competition">
        <rdfs:comment xml:lang="en">This frame is concerned with the idea that people (Participant1, Participant2, or Participants) participate in an organized rule governed activity (the Competition) in order to achieve some advantageous outcome (often the Prize). Rank and Score are different criteria by which the degree of achievement of the advantageous outcome is judged.  </rdfs:comment>
        <rdfs:label xml:lang="en">Competition</rdfs:label>
    </owl:Class>
    


    <!-- https://w3id.org/framester/data/framestercore/Supporting -->

    <owl:Class rdf:about="https://w3id.org/framester/data/framestercore/Supporting">
        <rdfs:comment xml:lang="en">A Supporter assists to strengthen the Supported by lending itself in material aid (or abstract assistance in the case of metaphorical uses). The bottom of the wall is supported by the foundation. Many legislators have supported the industry in the past. The revetment layers buttressed the mud-mortared cobblestone core wall. Online gambling can bolster the US economy.</rdfs:comment>
        <rdfs:label xml:lang="en">Supporting</rdfs:label>
    </owl:Class>
    


    <!-- https://w3id.org/framester/data/framestercore/Organization#SocialGroup -->

    <owl:Class rdf:about="https://w3id.org/framester/data/framestercore/Organization#SocialGroup">
        <rdfs:comment xml:lang="en">Represents a collection of individuals sharing common interests or affiliations.</rdfs:comment>
        <rdfs:label xml:lang="en">SocialGroup</rdfs:label>
    </owl:Class>
    


    <!-- 
    ///////////////////////////////////////////////////////////////////////////////////////
    //
    // Individuals
    //
    ///////////////////////////////////////////////////////////////////////////////////////
     -->

    


    <!-- https://raw.githubusercontent.com/Maedeam/KRKE-cognitive-biases/modeling-cognitive-biases/cognitive-biases/InGroupBias.owl#InterestCategory -->

    <owl:NamedIndividual rdf:about="https://raw.githubusercontent.com/Maedeam/KRKE-cognitive-biases/modeling-cognitive-biases/cognitive-biases/InGroupBias.owl#InterestCategory">
        <rdf:type rdf:resource="https://w3id.org/framester/data/framestercore/Categorization"/>
        <rdfs:comment xml:lang="en">Represents the category used to classify individuals within the social group.</rdfs:comment>
        <rdfs:label xml:lang="en">InterestCategory</rdfs:label>
    </owl:NamedIndividual>
    


    <!-- https://raw.githubusercontent.com/Maedeam/KRKE-cognitive-biases/modeling-cognitive-biases/cognitive-biases/InGroupBias.owl#John -->

    <owl:NamedIndividual rdf:about="https://raw.githubusercontent.com/Maedeam/KRKE-cognitive-biases/modeling-cognitive-biases/cognitive-biases/InGroupBias.owl#John">
        <rdf:type rdf:resource="http://www.ontologydesignpatterns.org/cp/owl/agentrole.owl#Agent"/>
        <rdf:type rdf:resource="http://www.ontologydesignpatterns.org/cp/owl/agentrole.owl#GroupMember"/>
        <rdfs:comment xml:lang="en">An individual who belongs to the Sports Fandom Group.</rdfs:comment>
        <rdfs:label xml:lang="en">John</rdfs:label>
    </owl:NamedIndividual>
    


    <!-- https://raw.githubusercontent.com/Maedeam/KRKE-cognitive-biases/modeling-cognitive-biases/cognitive-biases/InGroupBias.owl#SportsFandomGroup -->

    <owl:NamedIndividual rdf:about="https://raw.githubusercontent.com/Maedeam/KRKE-cognitive-biases/modeling-cognitive-biases/cognitive-biases/InGroupBias.owl#SportsFandomGroup">
        <rdf:type rdf:resource="https://w3id.org/framester/data/framestercore/Organization#SocialGroup"/>
        <rdfs:comment xml:lang="en">An instance of a social group formed around sports interests.</rdfs:comment>
        <rdfs:label xml:lang="en">SportsFandomGroup</rdfs:label>
    </owl:NamedIndividual>
</rdf:RDF>



<!-- Generated by the OWL API (version 4.5.26.2023-07-17T20:34:13Z) https://github.com/owlcs/owlapi -->

