<?xml version="1.0"?>
<rdf:RDF xmlns="http://www.semanticweb.org/delayed/cognitive-bias-ontology/HaloEffect#"
     xml:base="http://www.semanticweb.org/delayed/cognitive-bias-ontology/HaloEffect"
     xmlns:ns="http://creativecommons.org/ns#"
     xmlns:ns1="http://www.w3.org/2003/06/sw-vocab-status/ns#"
     xmlns:owl="http://www.w3.org/2002/07/owl#"
     xmlns:rdf="http://www.w3.org/1999/02/22-rdf-syntax-ns#"
     xmlns:xml="http://www.w3.org/XML/1998/namespace"
     xmlns:xsd="http://www.w3.org/2001/XMLSchema#"
     xmlns:rdfs="http://www.w3.org/2000/01/rdf-schema#"
     xmlns:vann="http://purl.org/vocab/vann/"
     xmlns:terms="http://purl.org/dc/terms/"
     xmlns:People="http://etna.istc.cnr.it/framester2/data/framestercore/People#"
     xmlns:HaloEffect="https://raw.githubusercontent.com/Maedeam/KRKE-cognitive-biases/modeling-cognitive-biases/cognitive-biases/Cluster1-FamiliarsBetterThanUnfamiliars/InGroupBias.owl#"
     xmlns:description="http://www.ontologydesignpatterns.org/cp/owl/description.owl#"
     xmlns:cpannotationschema="http://www.ontologydesignpatterns.org/schemas/cpannotationschema.owl#">
    <owl:Ontology rdf:about="https://raw.githubusercontent.com/Maedeam/KRKE-cognitive-biases/modeling-cognitive-biases/cognitive-biases/Cluster1-FamiliarsBetterThanUnfamiliars/InGroupBias.owl">
        <owl:versionIRI rdf:resource="https://raw.githubusercontent.com/Maedeam/KRKE-cognitive-biases/modeling-cognitive-biases/cognitive-biases/Cluster1-FamiliarsBetterThanUnfamiliars/InGroupBias.owl"/>
        <terms:creator xml:lang="en">Atousa Heidarnia</terms:creator>
        <terms:creator xml:lang="en">Maede Hajjari</terms:creator>
        <terms:description xml:lang="en">In Group Bias module of the Cognitive Bias Ontology</terms:description>
        <terms:hasVersion xml:lang="en">0.1</terms:hasVersion>
        <terms:title xml:lang="en">In Group Bias Ontology</terms:title>
        <rdfs:comment xml:lang="en">In-Group Bias, a prevalent cognitive bias, refers to the tendency of individuals to favor and show preferential treatment towards members of their own social, cultural, or identity group. This bias can lead to the perception of one&apos;s group as superior or more deserving than others, often resulting in a range of behaviors such as increased cooperation and empathy within the in-group and, conversely, discrimination or hostility towards out-groups. In-Group Bias is deeply rooted in social psychology, influencing how individuals perceive, interact with, and relate to those they consider part of their social circle.</rdfs:comment>
    </owl:Ontology>
    


    <!-- 
    ///////////////////////////////////////////////////////////////////////////////////////
    //
    // Annotation properties
    //
    ///////////////////////////////////////////////////////////////////////////////////////
     -->

    


    <!-- http://purl.org/dc/terms/creator -->

    <owl:AnnotationProperty rdf:about="http://purl.org/dc/terms/creator"/>
    


    <!-- http://purl.org/dc/terms/description -->

    <owl:AnnotationProperty rdf:about="http://purl.org/dc/terms/description"/>
    


    <!-- http://purl.org/dc/terms/hasVersion -->

    <owl:AnnotationProperty rdf:about="http://purl.org/dc/terms/hasVersion"/>
    


    <!-- http://purl.org/dc/terms/title -->

    <owl:AnnotationProperty rdf:about="http://purl.org/dc/terms/title"/>
    


    <!-- 
    ///////////////////////////////////////////////////////////////////////////////////////
    //
    // Object Properties
    //
    ///////////////////////////////////////////////////////////////////////////////////////
     -->

    


    <!-- http://etna.istc.cnr.it/framester2/data/framestercore/People#belongsToGroup -->

    <owl:ObjectProperty rdf:about="http://etna.istc.cnr.it/framester2/data/framestercore/People#belongsToGroup">
        <rdfs:domain rdf:resource="http://etna.istc.cnr.it/framester2/data/framestercore/People#GroupMember"/>
        <rdfs:range rdf:resource="http://etna.istc.cnr.it/framester2/data/framestercore/People#SocialGroup"/>
        <rdfs:comment xml:lang="en">Connects an individual to the social group they are a part of.</rdfs:comment>
        <rdfs:label xml:lang="en">belongsToGroup</rdfs:label>
    </owl:ObjectProperty>
    


    <!-- http://etna.istc.cnr.it/framester2/data/framestercore/People#exhibitsCategorization -->

    <owl:ObjectProperty rdf:about="http://etna.istc.cnr.it/framester2/data/framestercore/People#exhibitsCategorization">
        <rdfs:domain rdf:resource="http://etna.istc.cnr.it/framester2/data/framestercore/People#SocialGroup"/>
        <rdfs:range rdf:resource="http://etna.istc.cnr.it/framester2/data/framestercore/People#Categorization"/>
        <rdfs:comment xml:lang="en">Indicates the categorization process employed within a social group.</rdfs:comment>
        <rdfs:label xml:lang="en">exhibitsCategorization</rdfs:label>
    </owl:ObjectProperty>
    


    <!-- http://etna.istc.cnr.it/framester2/data/framestercore/People#hasBias -->

    <owl:ObjectProperty rdf:about="http://etna.istc.cnr.it/framester2/data/framestercore/People#hasBias">
        <rdfs:domain rdf:resource="http://etna.istc.cnr.it/framester2/data/framestercore/People#SocialGroup"/>
        <rdfs:range rdf:resource="http://etna.istc.cnr.it/framester2/data/framestercore/People#Bias"/>
        <rdfs:comment xml:lang="en">Relates a social group to the bias it exhibits towards its members.</rdfs:comment>
        <rdfs:label xml:lang="en">hasBias</rdfs:label>
    </owl:ObjectProperty>
    


    <!-- http://etna.istc.cnr.it/framester2/data/framestercore/People#hasName -->

    <owl:ObjectProperty rdf:about="http://etna.istc.cnr.it/framester2/data/framestercore/People#hasName">
        <rdfs:label xml:lang="en">hasName</rdfs:label>
    </owl:ObjectProperty>
    


    <!-- 
    ///////////////////////////////////////////////////////////////////////////////////////
    //
    // Classes
    //
    ///////////////////////////////////////////////////////////////////////////////////////
     -->

    


    <!-- http://etna.istc.cnr.it/framester2/data/framestercore/People#Bias -->

    <owl:Class rdf:about="http://etna.istc.cnr.it/framester2/data/framestercore/People#Bias">
        <rdfs:comment xml:lang="en">Represents the inclination or partiality towards certain individuals within a social group.</rdfs:comment>
        <rdfs:label xml:lang="en">Bias</rdfs:label>
    </owl:Class>
    


    <!-- http://etna.istc.cnr.it/framester2/data/framestercore/People#Categorization -->

    <owl:Class rdf:about="http://etna.istc.cnr.it/framester2/data/framestercore/People#Categorization">
        <rdfs:comment xml:lang="en">Represents the process of classifying individuals based on certain criteria.</rdfs:comment>
        <rdfs:label xml:lang="en">Categorization</rdfs:label>
    </owl:Class>
    


    <!-- http://etna.istc.cnr.it/framester2/data/framestercore/People#GroupMember -->

    <owl:Class rdf:about="http://etna.istc.cnr.it/framester2/data/framestercore/People#GroupMember">
        <rdfs:comment xml:lang="en">Represents an individual belonging to a social group.</rdfs:comment>
        <rdfs:label xml:lang="en">GroupMember</rdfs:label>
    </owl:Class>
    


    <!-- http://etna.istc.cnr.it/framester2/data/framestercore/People#SocialGroup -->

    <owl:Class rdf:about="http://etna.istc.cnr.it/framester2/data/framestercore/People#SocialGroup">
        <rdfs:comment xml:lang="en">Represents a collection of individuals sharing common interests or affiliations.</rdfs:comment>
        <rdfs:label xml:lang="en">SocialGroup</rdfs:label>
    </owl:Class>
    


    <!-- 
    ///////////////////////////////////////////////////////////////////////////////////////
    //
    // Individuals
    //
    ///////////////////////////////////////////////////////////////////////////////////////
     -->

    


    <!-- http://etna.istc.cnr.it/framester2/data/framestercore/People#InGroupBias -->

    <owl:NamedIndividual rdf:about="http://etna.istc.cnr.it/framester2/data/framestercore/People#InGroupBias">
        <rdf:type rdf:resource="http://etna.istc.cnr.it/framester2/data/framestercore/People#Bias"/>
        <People:belongsToGroup rdf:resource="http://etna.istc.cnr.it/framester2/data/framestercore/People#SportsFandomGroup"/>
        <People:exhibitsCategorization rdf:resource="http://etna.istc.cnr.it/framester2/data/framestercore/People#InterestCategory"/>
        <rdfs:comment xml:lang="en">An instance representing the bias towards individuals within a specific group.</rdfs:comment>
        <rdfs:label xml:lang="en">InGroupBias</rdfs:label>
    </owl:NamedIndividual>
    


    <!-- http://etna.istc.cnr.it/framester2/data/framestercore/People#InterestCategory -->

    <owl:NamedIndividual rdf:about="http://etna.istc.cnr.it/framester2/data/framestercore/People#InterestCategory">
        <rdf:type rdf:resource="http://etna.istc.cnr.it/framester2/data/framestercore/People#Categorization"/>
        <People:hasName rdf:resource="http://etna.istc.cnr.it/framester2/data/framestercore/People#Sports_Fandom"/>
        <rdfs:comment xml:lang="en">Represents the category used to classify individuals within the social group.</rdfs:comment>
        <rdfs:label xml:lang="en">InterestCategory</rdfs:label>
    </owl:NamedIndividual>
    


    <!-- http://etna.istc.cnr.it/framester2/data/framestercore/People#John -->

    <owl:NamedIndividual rdf:about="http://etna.istc.cnr.it/framester2/data/framestercore/People#John">
        <rdf:type rdf:resource="http://etna.istc.cnr.it/framester2/data/framestercore/People#GroupMember"/>
        <People:belongsToGroup rdf:resource="http://etna.istc.cnr.it/framester2/data/framestercore/People#SportsFandomGroup"/>
        <People:exhibitsCategorization rdf:resource="http://etna.istc.cnr.it/framester2/data/framestercore/People#InterestCategory"/>
        <People:hasBias rdf:resource="http://etna.istc.cnr.it/framester2/data/framestercore/People#InGroupBias"/>
        <rdfs:comment xml:lang="en">An individual who belongs to the Sports Fandom Group.</rdfs:comment>
        <rdfs:label xml:lang="en">John</rdfs:label>
    </owl:NamedIndividual>
    


    <!-- http://etna.istc.cnr.it/framester2/data/framestercore/People#Mary -->

    <owl:NamedIndividual rdf:about="http://etna.istc.cnr.it/framester2/data/framestercore/People#Mary">
        <rdf:type rdf:resource="http://etna.istc.cnr.it/framester2/data/framestercore/People#GroupMember"/>
        <People:belongsToGroup rdf:resource="http://etna.istc.cnr.it/framester2/data/framestercore/People#SportsFandomGroup"/>
        <rdfs:label xml:lang="en">Mary</rdfs:label>
    </owl:NamedIndividual>
    


    <!-- http://etna.istc.cnr.it/framester2/data/framestercore/People#SportsFandomGroup -->

    <owl:NamedIndividual rdf:about="http://etna.istc.cnr.it/framester2/data/framestercore/People#SportsFandomGroup">
        <rdf:type rdf:resource="http://etna.istc.cnr.it/framester2/data/framestercore/People#SocialGroup"/>
        <People:hasBias rdf:resource="http://etna.istc.cnr.it/framester2/data/framestercore/People#InGroupBias"/>
        <rdfs:comment xml:lang="en">An instance of a social group formed around sports interests.</rdfs:comment>
        <rdfs:label xml:lang="en">SportsFandomGroup</rdfs:label>
    </owl:NamedIndividual>
    


    <!-- http://etna.istc.cnr.it/framester2/data/framestercore/People#Sports_Fandom -->

    <owl:NamedIndividual rdf:about="http://etna.istc.cnr.it/framester2/data/framestercore/People#Sports_Fandom">
        <rdfs:label xml:lang="en">&quot;Sports Fandom&quot;</rdfs:label>
    </owl:NamedIndividual>
    


    <!-- 
    ///////////////////////////////////////////////////////////////////////////////////////
    //
    // Annotations
    //
    ///////////////////////////////////////////////////////////////////////////////////////
     -->

    <rdf:Description rdf:about="http://www.w3.org/2002/07/owl#deprecated">
        <rdfs:label xml:lang="en">Celebrity</rdfs:label>
    </rdf:Description>
</rdf:RDF>



<!-- Generated by the OWL API (version 4.5.26.2023-07-17T20:34:13Z) https://github.com/owlcs/owlapi -->
