<?xml version="1.0"?>
<rdf:RDF xmlns="http://www.semanticweb.org/delayed/cognitive-bias-ontology/NotInventedHere#"
     xml:base="http://www.semanticweb.org/delayed/cognitive-bias-ontology/NotInventedHere"
     xmlns:owl="http://www.w3.org/2002/07/owl#"
     xmlns:rdf="http://www.w3.org/1999/02/22-rdf-syntax-ns#"
     xmlns:xml="http://www.w3.org/XML/1998/namespace"
     xmlns:xsd="http://www.w3.org/2001/XMLSchema#"
     xmlns:rdfs="http://www.w3.org/2000/01/rdf-schema#"
     xmlns:terms="http://purl.org/dc/terms/"
     xmlns:NotInventedHere="http://www.semanticweb.org/delayed/cognitive-bias-ontology/NotInventedHere#"
     xmlns:NotInventedHere1="https://raw.githubusercontent.com/Maedeam/KRKE-cognitive-biases/modeling-cognitive-biases/cognitive-biases/NotInventedHere.owl#">
    <owl:Ontology rdf:about="https://raw.githubusercontent.com/Maedeam/KRKE-cognitive-biases/modeling-cognitive-biases/cognitive-biases/NotInventedHere.owl">
        <terms:creator xml:lang="en">Atousa Heidarnia</terms:creator>
        <terms:creator xml:lang="en">Maede Hajjari</terms:creator>
        <terms:description xml:lang="en">Not Invented Here module of the Cognitive Bias Ontology.</terms:description>
        <terms:hasVersion xml:lang="en">0.1</terms:hasVersion>
        <terms:title xml:lang="en">Not Invented Here Ontology</terms:title>
        <rdfs:comment xml:lang="en">&quot;Not Invented Here Bias&quot; is a cognitive bias characterized by a reluctance or skepticism towards adopting external ideas, products, or solutions, simply because they were not created internally. Individuals or organizations affected by this bias may undervalue or dismiss external innovations, preferring to rely on their own methods or developments. This bias can hinder progress, limit diversity of thought, and impede the adoption of valuable insights from external sources. Overcoming the &quot;Not Invented Here Bias&quot; involves fostering a more open-minded approach that appreciates external contributions and acknowledges the potential benefits of embracing ideas regardless of their origin.</rdfs:comment>
    </owl:Ontology>
    


    <!-- 
    ///////////////////////////////////////////////////////////////////////////////////////
    //
    // Annotation properties
    //
    ///////////////////////////////////////////////////////////////////////////////////////
     -->

    


    <!-- http://purl.org/dc/terms/creator -->

    <owl:AnnotationProperty rdf:about="http://purl.org/dc/terms/creator"/>
    


    <!-- http://purl.org/dc/terms/description -->

    <owl:AnnotationProperty rdf:about="http://purl.org/dc/terms/description"/>
    


    <!-- http://purl.org/dc/terms/hasVersion -->

    <owl:AnnotationProperty rdf:about="http://purl.org/dc/terms/hasVersion"/>
    


    <!-- http://purl.org/dc/terms/title -->

    <owl:AnnotationProperty rdf:about="http://purl.org/dc/terms/title"/>
    


    <!-- 
    ///////////////////////////////////////////////////////////////////////////////////////
    //
    // Object Properties
    //
    ///////////////////////////////////////////////////////////////////////////////////////
     -->

    


    <!-- https://raw.githubusercontent.com/Maedeam/KRKE-cognitive-biases/modeling-cognitive-biases/cognitive-biases/NotInventedHere.owl#dependsOn -->

    <owl:ObjectProperty rdf:about="https://raw.githubusercontent.com/Maedeam/KRKE-cognitive-biases/modeling-cognitive-biases/cognitive-biases/NotInventedHere.owl#dependsOn">
        <rdfs:domain rdf:resource="http://etna.istc.cnr.it/framester2/data/framestercore/Preference"/>
        <rdfs:range rdf:resource="http://etna.istc.cnr.it/framester2/data/framestercore/PartInnerOuter"/>
        <rdfs:comment xml:lang="en">Describe a dependency between to entities.</rdfs:comment>
        <rdfs:label xml:lang="en">dependsOn</rdfs:label>
    </owl:ObjectProperty>
    


    <!-- https://raw.githubusercontent.com/Maedeam/KRKE-cognitive-biases/modeling-cognitive-biases/cognitive-biases/NotInventedHere.owl#hasPartOrigin -->

    <owl:ObjectProperty rdf:about="https://raw.githubusercontent.com/Maedeam/KRKE-cognitive-biases/modeling-cognitive-biases/cognitive-biases/NotInventedHere.owl#hasPartOrigin">
        <rdfs:domain rdf:resource="http://etna.istc.cnr.it/framester2/data/framestercore/Creating"/>
        <rdfs:range rdf:resource="http://etna.istc.cnr.it/framester2/data/framestercore/PartInnerOuter"/>
        <rdfs:comment xml:lang="en">Represents the origin (internal or external) of parts in the creation process.</rdfs:comment>
        <rdfs:label xml:lang="en">hasPartOrigin</rdfs:label>
    </owl:ObjectProperty>
    


    <!-- https://raw.githubusercontent.com/Maedeam/KRKE-cognitive-biases/modeling-cognitive-biases/cognitive-biases/NotInventedHere.owl#hasPreference -->

    <owl:ObjectProperty rdf:about="https://raw.githubusercontent.com/Maedeam/KRKE-cognitive-biases/modeling-cognitive-biases/cognitive-biases/NotInventedHere.owl#hasPreference">
        <rdfs:domain rdf:resource="http://etna.istc.cnr.it/framester2/data/framestercore/Organization"/>
        <rdfs:domain rdf:resource="http://www.ontologydesignpatterns.org/cp/owl/agentrole.owl#GroupMember"/>
        <rdfs:range rdf:resource="http://etna.istc.cnr.it/framester2/data/framestercore/Preference"/>
        <rdfs:comment xml:lang="en">Represents the preference of an organization towards internal or external solutions.</rdfs:comment>
        <rdfs:label xml:lang="en">hasPreference</rdfs:label>
    </owl:ObjectProperty>
    


    <!-- https://w3id.org/affectedBy#affectedBy -->

    <owl:ObjectProperty rdf:about="https://w3id.org/affectedBy#affectedBy">
        <rdfs:domain rdf:resource="http://etna.istc.cnr.it/framester2/data/framestercore/Preference"/>
        <rdfs:range rdf:resource="http://etna.istc.cnr.it/framester2/data/framestercore/PartInnerOuter"/>
        <rdfs:comment xml:lang="en">A relation between qualities or entities.</rdfs:comment>
        <rdfs:label xml:lang="en">affectedBy</rdfs:label>
    </owl:ObjectProperty>
    


    <!-- https://w3id.org/affectedBy#belongsTo -->

    <owl:ObjectProperty rdf:about="https://w3id.org/affectedBy#belongsTo">
        <rdfs:domain rdf:resource="http://www.ontologydesignpatterns.org/cp/owl/agentrole.owl#GroupMember"/>
        <rdfs:range rdf:resource="http://etna.istc.cnr.it/framester2/data/framestercore/Organization"/>
        <rdfs:comment xml:lang="en">A relation between qualities and features of interest.</rdfs:comment>
        <rdfs:label xml:lang="en">belongsTo</rdfs:label>
    </owl:ObjectProperty>
    


    <!-- 
    ///////////////////////////////////////////////////////////////////////////////////////
    //
    // Classes
    //
    ///////////////////////////////////////////////////////////////////////////////////////
     -->

    


    <!-- http://etna.istc.cnr.it/framester2/data/framestercore/Creating -->

    <owl:Class rdf:about="http://etna.istc.cnr.it/framester2/data/framestercore/Creating">
        <rdfs:comment xml:lang="en">Represents the act of creating or developing.</rdfs:comment>
        <rdfs:label xml:lang="en">Creating</rdfs:label>
    </owl:Class>
    


    <!-- http://etna.istc.cnr.it/framester2/data/framestercore/Organization -->

    <owl:Class rdf:about="http://etna.istc.cnr.it/framester2/data/framestercore/Organization">
        <rdfs:comment xml:lang="en">Represents entities such as companies or teams</rdfs:comment>
        <rdfs:label xml:lang="en">Organization</rdfs:label>
    </owl:Class>
    


    <!-- http://etna.istc.cnr.it/framester2/data/framestercore/PartInnerOuter -->

    <owl:Class rdf:about="http://etna.istc.cnr.it/framester2/data/framestercore/PartInnerOuter">
        <rdfs:comment xml:lang="en">represents the relationship between parts and their internal or external origin</rdfs:comment>
        <rdfs:label xml:lang="en">PartInnerOuter</rdfs:label>
    </owl:Class>
    


    <!-- http://etna.istc.cnr.it/framester2/data/framestercore/Preference -->

    <owl:Class rdf:about="http://etna.istc.cnr.it/framester2/data/framestercore/Preference">
        <rdfs:comment xml:lang="en">Preference refers to a person&apos;s liking or inclination towards one option over another, often based on individual tastes, desires, or subjective judgments.</rdfs:comment>
        <rdfs:label xml:lang="en">Preference</rdfs:label>
    </owl:Class>
    


    <!-- http://www.ontologydesignpatterns.org/cp/owl/agentrole.owl#GroupMember -->

    <owl:Class rdf:about="http://www.ontologydesignpatterns.org/cp/owl/agentrole.owl#GroupMember">
        <rdfs:subClassOf rdf:resource="http://etna.istc.cnr.it/framester2/data/framestercore/Organization"/>
        <rdfs:comment xml:lang="en">Represents an individual belonging to a social group.</rdfs:comment>
        <rdfs:label xml:lang="en">GroupMember</rdfs:label>
    </owl:Class>
    


    <!-- 
    ///////////////////////////////////////////////////////////////////////////////////////
    //
    // Individuals
    //
    ///////////////////////////////////////////////////////////////////////////////////////
     -->

    


    <!-- https://raw.githubusercontent.com/Maedeam/KRKE-cognitive-biases/modeling-cognitive-biases/cognitive-biases/NotInventedHere.owl#ExternalInnovation -->

    <owl:NamedIndividual rdf:about="https://raw.githubusercontent.com/Maedeam/KRKE-cognitive-biases/modeling-cognitive-biases/cognitive-biases/NotInventedHere.owl#ExternalInnovation">
        <rdf:type rdf:resource="http://etna.istc.cnr.it/framester2/data/framestercore/Creating"/>
        <rdfs:comment xml:lang="en">An instance of Creating representing the act of developing external innovations.</rdfs:comment>
        <rdfs:label xml:lang="en">ExternalInnovation</rdfs:label>
    </owl:NamedIndividual>
    


    <!-- https://raw.githubusercontent.com/Maedeam/KRKE-cognitive-biases/modeling-cognitive-biases/cognitive-biases/NotInventedHere.owl#InternalSolutions -->

    <owl:NamedIndividual rdf:about="https://raw.githubusercontent.com/Maedeam/KRKE-cognitive-biases/modeling-cognitive-biases/cognitive-biases/NotInventedHere.owl#InternalSolutions">
        <rdf:type rdf:resource="http://etna.istc.cnr.it/framester2/data/framestercore/Creating"/>
        <rdfs:comment xml:lang="en">An instance of Preference representing a bias towards internal solutions.</rdfs:comment>
        <rdfs:label xml:lang="en">InternalSolutions</rdfs:label>
    </owl:NamedIndividual>
    


    <!-- https://raw.githubusercontent.com/Maedeam/KRKE-cognitive-biases/modeling-cognitive-biases/cognitive-biases/NotInventedHere.owl#ProductDevelopmentTeam -->

    <owl:NamedIndividual rdf:about="https://raw.githubusercontent.com/Maedeam/KRKE-cognitive-biases/modeling-cognitive-biases/cognitive-biases/NotInventedHere.owl#ProductDevelopmentTeam">
        <rdf:type rdf:resource="http://etna.istc.cnr.it/framester2/data/framestercore/Organization"/>
        <rdfs:comment xml:lang="en">An instance of Organization representing a team engaged in product development.</rdfs:comment>
        <rdfs:label xml:lang="en">ProductDevelopmentTeam</rdfs:label>
    </owl:NamedIndividual>
</rdf:RDF>



<!-- Generated by the OWL API (version 4.5.26.2023-07-17T20:34:13Z) https://github.com/owlcs/owlapi -->

