<?xml version="1.0"?>
<rdf:RDF xmlns="http://www.semanticweb.org/delayed/cognitive-bias-ontology/NotInventedHere#"
     xml:base="http://www.semanticweb.org/delayed/cognitive-bias-ontology/NotInventedHere"
     xmlns:ns="http://creativecommons.org/ns#"
     xmlns:ns1="http://www.w3.org/2003/06/sw-vocab-status/ns#"
     xmlns:owl="http://www.w3.org/2002/07/owl#"
     xmlns:rdf="http://www.w3.org/1999/02/22-rdf-syntax-ns#"
     xmlns:xml="http://www.w3.org/XML/1998/namespace"
     xmlns:xsd="http://www.w3.org/2001/XMLSchema#"
     xmlns:rdfs="http://www.w3.org/2000/01/rdf-schema#"
     xmlns:skos="http://www.w3.org/2004/02/skos/core#"
     xmlns:vann="http://purl.org/vocab/vann/"
     xmlns:terms="http://purl.org/dc/terms/"
     xmlns:NotInventedHere="https://raw.githubusercontent.com/Maedeam/KRKE-cognitive-biases/modeling-cognitive-biases/cognitive-biases/NotInventedHere.owl"
     xmlns:description="http://www.ontologydesignpatterns.org/cp/owl/description.owl#"
     xmlns:NotInventedHere1="https://raw.githubusercontent.com/Maedeam/KRKE-cognitive-biases/modeling-cognitive-biases/cognitive-biases/NotInventedHere.owl#"
     xmlns:NotInventedHere2="https://raw.githubusercontent.com/Maedeam/KRKE-cognitive-biases/modeling-cognitive-biases/cognitive-biases/NotInventedHere#"
     xmlns:cpannotationschema="http://www.ontologydesignpatterns.org/schemas/cpannotationschema.owl#">
    <owl:Ontology rdf:about="https://raw.githubusercontent.com/Maedeam/KRKE-cognitive-biases/modeling-cognitive-biases/cognitive-biases/NotInventedHere.owl">
        <owl:versionIRI rdf:resource="https://raw.githubusercontent.com/Maedeam/KRKE-cognitive-biases/modeling-cognitive-biases/cognitive-biases/NotInventedHere.owl"/>
        <terms:creator xml:lang="en">Atousa Heidarnia</terms:creator>
        <terms:creator xml:lang="en">Maede Hajjari</terms:creator>
        <terms:description xml:lang="en">Not Invented Here module of the Cognitive Bias Ontology.</terms:description>
        <terms:hasVersion xml:lang="en">0.1</terms:hasVersion>
        <terms:title xml:lang="en">Not Invented Here Ontology</terms:title>
        <rdfs:comment xml:lang="en">&quot;Not Invented Here Bias&quot; is a cognitive bias characterized by a reluctance or skepticism towards adopting external ideas, products, or solutions, simply because they were not created internally. Individuals or organizations affected by this bias may undervalue or dismiss external innovations, preferring to rely on their own methods or developments. This bias can hinder progress, limit diversity of thought, and impede the adoption of valuable insights from external sources. Overcoming the &quot;Not Invented Here Bias&quot; involves fostering a more open-minded approach that appreciates external contributions and acknowledges the potential benefits of embracing ideas regardless of their origin.</rdfs:comment>
    </owl:Ontology>
    


    <!-- 
    ///////////////////////////////////////////////////////////////////////////////////////
    //
    // Annotation properties
    //
    ///////////////////////////////////////////////////////////////////////////////////////
     -->

    


    <!-- http://purl.org/dc/terms/creator -->

    <owl:AnnotationProperty rdf:about="http://purl.org/dc/terms/creator"/>
    


    <!-- http://purl.org/dc/terms/description -->

    <owl:AnnotationProperty rdf:about="http://purl.org/dc/terms/description"/>
    


    <!-- http://purl.org/dc/terms/hasVersion -->

    <owl:AnnotationProperty rdf:about="http://purl.org/dc/terms/hasVersion"/>
    


    <!-- http://purl.org/dc/terms/title -->

    <owl:AnnotationProperty rdf:about="http://purl.org/dc/terms/title"/>
    


    <!-- http://www.w3.org/2004/02/skos/core#comment -->

    <owl:AnnotationProperty rdf:about="http://www.w3.org/2004/02/skos/core#comment"/>
    


    <!-- 
    ///////////////////////////////////////////////////////////////////////////////////////
    //
    // Object Properties
    //
    ///////////////////////////////////////////////////////////////////////////////////////
     -->

    


    <!-- https://raw.githubusercontent.com/Maedeam/KRKE-cognitive-biases/modeling-cognitive-biases/cognitive-biases/NotInventedHere#develops -->

    <owl:ObjectProperty rdf:about="https://raw.githubusercontent.com/Maedeam/KRKE-cognitive-biases/modeling-cognitive-biases/cognitive-biases/NotInventedHere#develops">
        <rdfs:domain rdf:resource="http://etna.istc.cnr.it/framester2/data/framestercore/Partiality#Organization"/>
        <rdfs:range rdf:resource="http://etna.istc.cnr.it/framester2/data/framestercore/Categorization#Creating"/>
        <rdfs:comment xml:lang="en">Represents the act of an organization creating solutions.</rdfs:comment>
        <rdfs:label xml:lang="en">develops</rdfs:label>
    </owl:ObjectProperty>
    


    <!-- https://raw.githubusercontent.com/Maedeam/KRKE-cognitive-biases/modeling-cognitive-biases/cognitive-biases/NotInventedHere#hasPartOrigin -->

    <owl:ObjectProperty rdf:about="https://raw.githubusercontent.com/Maedeam/KRKE-cognitive-biases/modeling-cognitive-biases/cognitive-biases/NotInventedHere#hasPartOrigin">
        <rdfs:domain rdf:resource="http://etna.istc.cnr.it/framester2/data/framestercore/Categorization#Creating"/>
        <rdfs:range rdf:resource="https://raw.githubusercontent.com/Maedeam/KRKE-cognitive-biases/modeling-cognitive-biases/cognitive-biases/NotInventedHere#PartInnerOuter"/>
        <rdfs:comment xml:lang="en">Represents the origin (internal or external) of parts in the creation process.</rdfs:comment>
        <rdfs:label xml:lang="en">hasPartOrigin</rdfs:label>
    </owl:ObjectProperty>
    


    <!-- https://raw.githubusercontent.com/Maedeam/KRKE-cognitive-biases/modeling-cognitive-biases/cognitive-biases/NotInventedHere#hasPreference -->

    <owl:ObjectProperty rdf:about="https://raw.githubusercontent.com/Maedeam/KRKE-cognitive-biases/modeling-cognitive-biases/cognitive-biases/NotInventedHere#hasPreference">
        <rdfs:domain rdf:resource="http://etna.istc.cnr.it/framester2/data/framestercore/Partiality#Organization"/>
        <rdfs:range rdf:resource="http://etna.istc.cnr.it/framester2/data/framestercore/Preference"/>
        <rdfs:comment xml:lang="en">Represents the preference of an organization towards internal or external solutions.</rdfs:comment>
        <rdfs:label xml:lang="en">hasPreference</rdfs:label>
    </owl:ObjectProperty>
    


    <!-- 
    ///////////////////////////////////////////////////////////////////////////////////////
    //
    // Classes
    //
    ///////////////////////////////////////////////////////////////////////////////////////
     -->

    


    <!-- http://etna.istc.cnr.it/framester2/data/framestercore/Preference -->

    <owl:Class rdf:about="http://etna.istc.cnr.it/framester2/data/framestercore/Preference">
        <rdfs:comment xml:lang="en">Represents the inclination or bias towards internal solutions</rdfs:comment>
        <rdfs:label xml:lang="en">Preference</rdfs:label>
    </owl:Class>
    


    <!-- http://etna.istc.cnr.it/framester2/data/framestercore/Categorization#Creating -->

    <owl:Class rdf:about="http://etna.istc.cnr.it/framester2/data/framestercore/Categorization#Creating">
        <rdfs:comment xml:lang="en">Represents the act of creating or developing solutions.</rdfs:comment>
        <rdfs:label xml:lang="en">Creating</rdfs:label>
    </owl:Class>
    


    <!-- http://etna.istc.cnr.it/framester2/data/framestercore/Categorization#PartInnerOuter -->

    <owl:Class rdf:about="http://etna.istc.cnr.it/framester2/data/framestercore/Categorization#PartInnerOuter">
        <rdfs:comment xml:lang="en">Represents the relationship between parts and their internal or external origin.</rdfs:comment>
        <rdfs:label xml:lang="en">GroupMember</rdfs:label>
    </owl:Class>
    


    <!-- http://etna.istc.cnr.it/framester2/data/framestercore/Partiality#Organization -->

    <owl:Class rdf:about="http://etna.istc.cnr.it/framester2/data/framestercore/Partiality#Organization">
        <rdfs:comment xml:lang="en">Represents entities such as companies or teams</rdfs:comment>
        <rdfs:label xml:lang="en">Organization</rdfs:label>
    </owl:Class>
    


    <!-- https://raw.githubusercontent.com/Maedeam/KRKE-cognitive-biases/modeling-cognitive-biases/cognitive-biases/NotInventedHere#PartInnerOuter -->

    <owl:Class rdf:about="https://raw.githubusercontent.com/Maedeam/KRKE-cognitive-biases/modeling-cognitive-biases/cognitive-biases/NotInventedHere#PartInnerOuter">
        <rdfs:comment xml:lang="en">represents the relationship between parts and their internal or external origin</rdfs:comment>
        <rdfs:label xml:lang="en">PartInnerOuter</rdfs:label>
    </owl:Class>
    


    <!-- 
    ///////////////////////////////////////////////////////////////////////////////////////
    //
    // Individuals
    //
    ///////////////////////////////////////////////////////////////////////////////////////
     -->

    


    <!-- https://raw.githubusercontent.com/Maedeam/KRKE-cognitive-biases/modeling-cognitive-biases/cognitive-biases/NotInventedHere#ExternalInnovation -->

    <owl:NamedIndividual rdf:about="https://raw.githubusercontent.com/Maedeam/KRKE-cognitive-biases/modeling-cognitive-biases/cognitive-biases/NotInventedHere#ExternalInnovation">
        <rdf:type rdf:resource="http://etna.istc.cnr.it/framester2/data/framestercore/Categorization#Creating"/>
        <rdfs:comment xml:lang="en">An instance of Creating representing the act of developing external innovations.</rdfs:comment>
        <rdfs:label xml:lang="en">ExternalInnovation</rdfs:label>
    </owl:NamedIndividual>
    


    <!-- https://raw.githubusercontent.com/Maedeam/KRKE-cognitive-biases/modeling-cognitive-biases/cognitive-biases/NotInventedHere#InternalSolutions -->

    <owl:NamedIndividual rdf:about="https://raw.githubusercontent.com/Maedeam/KRKE-cognitive-biases/modeling-cognitive-biases/cognitive-biases/NotInventedHere#InternalSolutions">
        <rdf:type rdf:resource="http://etna.istc.cnr.it/framester2/data/framestercore/Preference"/>
        <NotInventedHere2:develops rdf:resource="https://raw.githubusercontent.com/Maedeam/KRKE-cognitive-biases/modeling-cognitive-biases/cognitive-biases/NotInventedHere#ExternalInnovation"/>
        <rdfs:comment xml:lang="en">An instance of Preference representing a bias towards internal solutions.</rdfs:comment>
        <rdfs:label xml:lang="en">InternalSolutions</rdfs:label>
    </owl:NamedIndividual>
    


    <!-- https://raw.githubusercontent.com/Maedeam/KRKE-cognitive-biases/modeling-cognitive-biases/cognitive-biases/NotInventedHere#ProductDevelopmentTeam -->

    <owl:NamedIndividual rdf:about="https://raw.githubusercontent.com/Maedeam/KRKE-cognitive-biases/modeling-cognitive-biases/cognitive-biases/NotInventedHere#ProductDevelopmentTeam">
        <rdf:type rdf:resource="http://etna.istc.cnr.it/framester2/data/framestercore/Partiality#Organization"/>
        <NotInventedHere2:hasPreference rdf:resource="https://raw.githubusercontent.com/Maedeam/KRKE-cognitive-biases/modeling-cognitive-biases/cognitive-biases/NotInventedHere#InternalSolutions"/>
        <rdfs:comment xml:lang="en">An instance of Organization representing a team engaged in product development.</rdfs:comment>
        <rdfs:label xml:lang="en">ProductDevelopmentTeam</rdfs:label>
    </owl:NamedIndividual>
</rdf:RDF>



<!-- Generated by the OWL API (version 4.5.26.2023-07-17T20:34:13Z) https://github.com/owlcs/owlapi -->
