<?xml version="1.0"?>
<rdf:RDF xmlns="http://www.semanticweb.org/delayed/cognitive-bias-ontology/welltraveledroadeffect#"
     xml:base="http://www.semanticweb.org/delayed/cognitive-bias-ontology/welltraveledroadeffect"
     xmlns:ns="http://creativecommons.org/ns#"
     xmlns:ns1="http://www.w3.org/2003/06/sw-vocab-status/ns#"
     xmlns:owl="http://www.w3.org/2002/07/owl#"
     xmlns:rdf="http://www.w3.org/1999/02/22-rdf-syntax-ns#"
     xmlns:xml="http://www.w3.org/XML/1998/namespace"
     xmlns:xsd="http://www.w3.org/2001/XMLSchema#"
     xmlns:rdfs="http://www.w3.org/2000/01/rdf-schema#"
     xmlns:vann="http://purl.org/vocab/vann/"
     xmlns:terms="http://purl.org/dc/terms/"
     xmlns:HaloEffect="https://raw.githubusercontent.com/Maedeam/KRKE-cognitive-biases/modeling-cognitive-biases/cognitive-biases/welltraveledroadeffect.owl"
     xmlns:HaloEffect1="https://raw.githubusercontent.com/Maedeam/KRKE-cognitive-biases/modeling-cognitive-biases/cognitive-biases/welltraveledroadeffect.owl#"
     xmlns:description="http://www.ontologydesignpatterns.org/cp/owl/description.owl#"
     xmlns:cpannotationschema="http://www.ontologydesignpatterns.org/schemas/cpannotationschema.owl#">
    <owl:Ontology rdf:about="https://raw.githubusercontent.com/Maedeam/KRKE-cognitive-biases/modeling-cognitive-biases/cognitive-biases/welltraveledroadeffect.owl">
        <owl:versionIRI rdf:resource="https://raw.githubusercontent.com/Maedeam/KRKE-cognitive-biases/modeling-cognitive-biases/cognitive-biases/welltraveledroadeffect.owl"/>
        <terms:creator xml:lang="en">Atousa Heidarnia</terms:creator>
        <terms:creator xml:lang="en">Maede Hajjari</terms:creator>
        <terms:description xml:lang="en">well-traveled road effect module of the Cognitive Bias Ontology.</terms:description>
        <terms:hasVersion xml:lang="en">0.1</terms:hasVersion>
        <terms:title xml:lang="en">well-traveled road effect Ontology</terms:title>
        <rdfs:comment xml:lang="en">The &quot;well-traveled road effect&quot;refers to the tendency of individuals to prefer familiar or conventional choices over novel alternatives.</rdfs:comment>
    </owl:Ontology>
    

    <!-- 
    ///////////////////////////////////////////////////////////////////////////////////////
    //
    // Object Properties
    //
    ///////////////////////////////////////////////////////////////////////////////////////
     -->

    


    <!-- http://webprotege.stanford.edu/R9SDNdxNVX8TV5bSOBcSMvO -->

    <owl:ObjectProperty rdf:about="http://webprotege.stanford.edu/R9SDNdxNVX8TV5bSOBcSMvO">
        <rdfs:subPropertyOf rdf:resource="http://www.w3.org/2002/07/owl#topObjectProperty"/>
        <rdfs:domain rdf:resource="http://webprotege.stanford.edu/RBa2rcC7eyhMdGCIaifal4I"/>
        <rdfs:range rdf:resource="http://webprotege.stanford.edu/RX6SeiBxVQopXEEy7yLN7D"/>
        <rdfs:comment rdf:datatype="http://www.w3.org/2001/XMLSchema#string">Relates individuals or teams to the project management methodology they choose to adopt, reflecting the decision-making process and the impact of the &quot;well-traveled road effect.&quot;</rdfs:comment>
        <rdfs:label xml:lang="en">AdoptsMethodology</rdfs:label>
    </owl:ObjectProperty>
    


    <!-- http://webprotege.stanford.edu/R9WrcTLV0Kw0JX8C16S0ziT -->

    <owl:ObjectProperty rdf:about="http://webprotege.stanford.edu/R9WrcTLV0Kw0JX8C16S0ziT">
        <rdfs:subPropertyOf rdf:resource="http://www.w3.org/2002/07/owl#topObjectProperty"/>
        <rdfs:domain rdf:resource="http://webprotege.stanford.edu/RBa2rcC7eyhMdGCIaifal4I"/>
        <rdfs:range rdf:resource="http://webprotege.stanford.edu/RDqxYCwHSEbFYJMss9xGLjO"/>
        <rdfs:comment rdf:datatype="http://www.w3.org/2001/XMLSchema#string">Links individuals or teams to their leadership style, whether it&apos;s proactive, reactive, or a combination, illustrating the role of leadership in navigating the &quot;well-traveled road effect.&quot;</rdfs:comment>
        <rdfs:label xml:lang="en">DemonstratesLeadershipStyle</rdfs:label>
    </owl:ObjectProperty>
    


    <!-- http://webprotege.stanford.edu/RBPWtw8Fouw9qdf46HA2Vyj -->

    <owl:ObjectProperty rdf:about="http://webprotege.stanford.edu/RBPWtw8Fouw9qdf46HA2Vyj">
        <rdfs:subPropertyOf rdf:resource="http://www.w3.org/2002/07/owl#topObjectProperty"/>
        <rdfs:domain rdf:resource="http://webprotege.stanford.edu/RBa2rcC7eyhMdGCIaifal4I"/>
        <rdfs:range rdf:resource="http://webprotege.stanford.edu/RX6SeiBxVQopXEEy7yLN7D"/>
        <rdfs:comment rdf:datatype="http://www.w3.org/2001/XMLSchema#string">A relationship highlighting how leadership styles can influence the decision to adopt a particular methodology, showcasing the impact on decision-making in the face of the well-traveled road effect.</rdfs:comment>
        <rdfs:label xml:lang="en">LeadershipInfluencesMethodologyChoice</rdfs:label>
    </owl:ObjectProperty>
    


    <!-- http://webprotege.stanford.edu/RDiL5sZ1o40YzLwh4enTx42 -->

    <owl:ObjectProperty rdf:about="http://webprotege.stanford.edu/RDiL5sZ1o40YzLwh4enTx42">
        <rdfs:subPropertyOf rdf:resource="http://www.w3.org/2002/07/owl#topObjectProperty"/>
        <rdfs:domain rdf:resource="http://webprotege.stanford.edu/RBa2rcC7eyhMdGCIaifal4I"/>
        <rdfs:range rdf:resource="http://webprotege.stanford.edu/RCeXEbZ7iheanb45hR5Lh2W"/>
        <rdfs:comment rdf:datatype="http://www.w3.org/2001/XMLSchema#string">Connects individuals or teams to challenges or dilemmas they encounter, emphasizing the difficulties associated with deviating from familiar paths and embracing change.</rdfs:comment>
        <rdfs:label xml:lang="en">FacesChallenge</rdfs:label>
    </owl:ObjectProperty>
    


    <!-- 
    ///////////////////////////////////////////////////////////////////////////////////////
    //
    // Classes
    //
    ///////////////////////////////////////////////////////////////////////////////////////
     -->



    <owl:Class rdf:about="https://w3id.org/framester/data/framestercore/People">
        <rdfs:subClassOf rdf:resource="https://w3id.org/framester/data/framestercore/Entity"/>
        <rdfs:comment>Represents individual professionals.</rdfs:comment>
        <rdfs:label xml:lang="en">Individuals</rdfs:label>
    </owl:Class>
    



    <owl:Class rdf:about="https://w3id.org/framester/data/framestercore/Expertise">
        <rdfs:subClassOf rdf:resource="https://w3id.org/framester/data/framestercore/Fields"/>
        <rdfs:comment>Represents the Agile project management methodology known for its flexibility and iterative approach.</rdfs:comment>
        <rdfs:label xml:lang="en">AgileMethodologies</rdfs:label>
    </owl:Class>
    


    <owl:Class rdf:about="https://w3id.org/framester/data/framestercore/Domain">
        <rdfs:subClassOf rdf:resource="https://w3id.org/framester/data/framestercore/Entity"/>
        <rdfs:comment>Represents specific roles that individuals may take on in a project.</rdfs:comment>
        <rdfs:label xml:lang="en">Roles</rdfs:label>
    </owl:Class>
    


    <owl:Class rdf:about="https://w3id.org/framester/data/framestercore/Organization">
        <rdfs:subClassOf rdf:resource="https://w3id.org/framester/data/framestercore/Entity"/>
        <rdfs:comment>Represents groups of individuals working together.</rdfs:comment>
        <rdfs:label xml:lang="en">Teams</rdfs:label>
    </owl:Class>
    

    <owl:Class rdf:about="https://w3id.org/framester/data/framestercore/MentalProperty">
        <rdfs:subClassOf rdf:resource="https://w3id.org/framester/data/framestercore/Entity"/>
        <rdfs:comment>Represents the overarching challenge faced by individuals or teams when deciding between established, well-known practices and innovative, less-explored alternatives.</rdfs:comment>
        <rdfs:label xml:lang="en">InnovationDilemma</rdfs:label>
    </owl:Class>
    


    <owl:Class rdf:about="https://w3id.org/framester/data/framestercore/Statement">
        <rdfs:subClassOf rdf:resource="https://w3id.org/framester/data/framestercore/Fields"/>
        <rdfs:comment>Represents the Traditional Waterfall project management methodology known for its linear and sequential approach.</rdfs:comment>
        <rdfs:label xml:lang="en">TraditionalWaterfallApproach</rdfs:label>
    </owl:Class>
    


    <owl:Class rdf:about="https://w3id.org/framester/data/framestercore/Leadership">
        <rdfs:subClassOf rdf:resource="https://w3id.org/framester/data/framestercore/Entity"/>
        <rdfs:comment>Encompasses different approaches to leadership, such as proactive leadership demonstrated by individuals like Emily, who actively seeks innovative solutions and challenges the status quo.</rdfs:comment>
        <rdfs:label xml:lang="en">LeadershipStyle</rdfs:label>
    </owl:Class>
    




    <owl:Class rdf:about="https://w3id.org/framester/data/framestercore/Entity">
        <rdfs:comment>A main class representing both individuals and teams in a professional setting.</rdfs:comment>
        <rdfs:label xml:lang="en">Entities</rdfs:label>
    </owl:Class>
    

    <owl:Class rdf:about="https://w3id.org/framester/data/framestercore/Fields">
        <rdfs:subClassOf rdf:resource="https://w3id.org/framester/data/framestercore/Entity"/>
        <rdfs:comment>Includes classes for different project management methodologies, like &quot;Agile Methodologies&quot; and &quot;Traditional Waterfall Approach,&quot; highlighting the paths that individuals or teams may choose.</rdfs:comment>
        <rdfs:label xml:lang="en">MethodologyParadigm</rdfs:label>
    </owl:Class>
    


    <!-- 
    ///////////////////////////////////////////////////////////////////////////////////////
    //
    // Individuals
    //
    ///////////////////////////////////////////////////////////////////////////////////////
     -->

    

    <owl:NamedIndividual rdf:about="https://w3id.org/framester/data/framestercore/People">
        <rdfs:comment>Represents an individual with the role of a project manager.</rdfs:comment>
        <rdfs:label xml:lang="en">ProjectManager</rdfs:label>
    </owl:NamedIndividual>
    


    <owl:NamedIndividual rdf:about="https://w3id.org/framester/data/framestercore/People">
        <rdfs:comment>Represents an individual with the role of a team member.</rdfs:comment>
        <rdfs:label xml:lang="en">TeamMember</rdfs:label>
    </owl:NamedIndividual>
</rdf:RDF>



<!-- Generated by the OWL API (version 4.5.13) https://github.com/owlcs/owlapi -->

