<?xml version="1.0"?>
<rdf:RDF xmlns="http://www.semanticweb.org/delayed/cognitive-bias-ontology/ImplicitAssociationss#"
     xml:base="http://www.semanticweb.org/delayed/cognitive-bias-ontology/ImplicitAssociationss"
     xmlns:ns="http://creativecommons.org/ns#"
     xmlns:ns1="http://www.w3.org/2003/06/sw-vocab-status/ns#"
     xmlns:owl="http://www.w3.org/2002/07/owl#"
     xmlns:rdf="http://www.w3.org/1999/02/22-rdf-syntax-ns#"
     xmlns:xml="http://www.w3.org/XML/1998/namespace"
     xmlns:xsd="http://www.w3.org/2001/XMLSchema#"
     xmlns:rdfs="http://www.w3.org/2000/01/rdf-schema#"
     xmlns:skos="http://www.w3.org/2004/02/skos/core#"
     xmlns:vann="http://purl.org/vocab/vann/"
     xmlns:terms="http://purl.org/dc/terms/"
     xmlns:description="http://www.ontologydesignpatterns.org/cp/owl/description.owl#"
     xmlns:cognitive-biases="https://raw.githubusercontent.com/Maedeam/KRKE-cognitive-biases/modeling-cognitive-biases/cognitive-biases/"
     xmlns:cpannotationschema="http://www.ontologydesignpatterns.org/schemas/cpannotationschema.owl#"
     xmlns:ImplicitAssociationss="https://raw.githubusercontent.com/Maedeam/KRKE-cognitive-biases/modeling-cognitive-biases/cognitive-biases/ImplicitAssociationss.owl"
     xmlns:ImplicitAssociationss1="https://raw.githubusercontent.com/Maedeam/KRKE-cognitive-biases/modeling-cognitive-biases/cognitive-biases/ImplicitAssociationss.owl#"
     xmlns:ImplicitAssociationss2="https://raw.githubusercontent.com/Maedeam/KRKE-cognitive-biases/modeling-cognitive-biases/cognitive-biases/ImplicitAssociationss#">
    <owl:Ontology rdf:about="https://raw.githubusercontent.com/Maedeam/KRKE-cognitive-biases/modeling-cognitive-biases/cognitive-biases/ImplicitAssociationss.owl">
        <owl:versionIRI rdf:resource="https://raw.githubusercontent.com/Maedeam/KRKE-cognitive-biases/modeling-cognitive-biases/cognitive-biases/ImplicitAssociationss.owl"/>
        <terms:creator xml:lang="en">Atousa Heidarnia</terms:creator>
        <terms:creator xml:lang="en">Maede Hajjari</terms:creator>
        <terms:description xml:lang="en">Implicit Associationss module of the Cognitive Bias Ontology.</terms:description>
        <terms:hasVersion xml:lang="en">0.1</terms:hasVersion>
        <terms:title xml:lang="en">Implicit Associationss Ontology</terms:title>
        <rdfs:comment xml:lang="en">Implicit Associations Bias refers to the unconscious and automatic associations or attitudes individuals hold toward certain groups or categories, influencing their judgments and behavior without conscious awareness. These biases are often deeply ingrained in societal norms and cultural contexts, shaping perceptions based on characteristics such as gender, race, or ethnicity. Implicit Associationss can affect decision-making processes, interactions, and evaluations, even when individuals consciously reject or oppose such biases. Recognizing and addressing Implicit Associations bias is crucial for promoting fairness, inclusivity, and equitable treatment in various social settings.</rdfs:comment>
    </owl:Ontology>
    


    <!-- 
    ///////////////////////////////////////////////////////////////////////////////////////
    //
    // Annotation properties
    //
    ///////////////////////////////////////////////////////////////////////////////////////
     -->

    


    <!-- http://purl.org/dc/terms/creator -->

    <owl:AnnotationProperty rdf:about="http://purl.org/dc/terms/creator"/>
    


    <!-- http://purl.org/dc/terms/description -->

    <owl:AnnotationProperty rdf:about="http://purl.org/dc/terms/description"/>
    


    <!-- http://purl.org/dc/terms/hasVersion -->

    <owl:AnnotationProperty rdf:about="http://purl.org/dc/terms/hasVersion"/>
    


    <!-- http://purl.org/dc/terms/title -->

    <owl:AnnotationProperty rdf:about="http://purl.org/dc/terms/title"/>
    


    <!-- http://www.w3.org/2004/02/skos/core#comment -->

    <owl:AnnotationProperty rdf:about="http://www.w3.org/2004/02/skos/core#comment"/>
    


    <!-- https://raw.githubusercontent.com/Maedeam/KRKE-cognitive-biases/modeling-cognitive-biases/cognitive-biases/ImplicitAssociationsBias.challengesBias -->

    <owl:AnnotationProperty rdf:about="https://raw.githubusercontent.com/Maedeam/KRKE-cognitive-biases/modeling-cognitive-biases/cognitive-biases/ImplicitAssociationsBias.challengesBias"/>
    


    <!-- https://raw.githubusercontent.com/Maedeam/KRKE-cognitive-biases/modeling-cognitive-biases/cognitive-biases/ImplicitAssociationsBias.exhibitsBiasTowards -->

    <owl:AnnotationProperty rdf:about="https://raw.githubusercontent.com/Maedeam/KRKE-cognitive-biases/modeling-cognitive-biases/cognitive-biases/ImplicitAssociationsBias.exhibitsBiasTowards"/>
    


    <!-- https://raw.githubusercontent.com/Maedeam/KRKE-cognitive-biases/modeling-cognitive-biases/cognitive-biases/ImplicitAssociationsBias.hasAttribute -->

    <owl:AnnotationProperty rdf:about="https://raw.githubusercontent.com/Maedeam/KRKE-cognitive-biases/modeling-cognitive-biases/cognitive-biases/ImplicitAssociationsBias.hasAttribute"/>
    


    <!-- https://raw.githubusercontent.com/Maedeam/KRKE-cognitive-biases/modeling-cognitive-biases/cognitive-biases/ImplicitAssociationss.owlchallengesBias -->

    <owl:AnnotationProperty rdf:about="https://raw.githubusercontent.com/Maedeam/KRKE-cognitive-biases/modeling-cognitive-biases/cognitive-biases/ImplicitAssociationss.owlchallengesBias"/>
    


    <!-- https://raw.githubusercontent.com/Maedeam/KRKE-cognitive-biases/modeling-cognitive-biases/cognitive-biases/ImplicitAssociationss.owlexhibitsBiasTowards -->

    <owl:AnnotationProperty rdf:about="https://raw.githubusercontent.com/Maedeam/KRKE-cognitive-biases/modeling-cognitive-biases/cognitive-biases/ImplicitAssociationss.owlexhibitsBiasTowards"/>
    


    <!-- https://raw.githubusercontent.com/Maedeam/KRKE-cognitive-biases/modeling-cognitive-biases/cognitive-biases/ImplicitAssociationss.owlhasAttribute -->

    <owl:AnnotationProperty rdf:about="https://raw.githubusercontent.com/Maedeam/KRKE-cognitive-biases/modeling-cognitive-biases/cognitive-biases/ImplicitAssociationss.owlhasAttribute"/>
    


    <!-- 
    ///////////////////////////////////////////////////////////////////////////////////////
    //
    // Object Properties
    //
    ///////////////////////////////////////////////////////////////////////////////////////
     -->

    


    <!-- https://raw.githubusercontent.com/Maedeam/KRKE-cognitive-biases/modeling-cognitive-biases/cognitive-biases/ImplicitAssociationss#challengesBias -->

    <owl:ObjectProperty rdf:about="https://raw.githubusercontent.com/Maedeam/KRKE-cognitive-biases/modeling-cognitive-biases/cognitive-biases/ImplicitAssociationss#challengesBias">
        <rdfs:domain rdf:resource="https://raw.githubusercontent.com/Maedeam/KRKE-cognitive-biases/modeling-cognitive-biases/cognitive-biases/ImplicitAssociationss#Person"/>
        <rdfs:range rdf:resource="https://raw.githubusercontent.com/Maedeam/KRKE-cognitive-biases/modeling-cognitive-biases/cognitive-biases/ImplicitAssociationss#ChallengeAction"/>
        <rdfs:comment xml:lang="en">Represents actions or behaviors that challenge or confront Implicit Associations Bias.</rdfs:comment>
        <rdfs:label xml:lang="en">challengesBias</rdfs:label>
    </owl:ObjectProperty>
    


    <!-- https://raw.githubusercontent.com/Maedeam/KRKE-cognitive-biases/modeling-cognitive-biases/cognitive-biases/ImplicitAssociationss#exhibitsBiasTowards -->

    <owl:ObjectProperty rdf:about="https://raw.githubusercontent.com/Maedeam/KRKE-cognitive-biases/modeling-cognitive-biases/cognitive-biases/ImplicitAssociationss#exhibitsBiasTowards">
        <rdfs:domain rdf:resource="https://raw.githubusercontent.com/Maedeam/KRKE-cognitive-biases/modeling-cognitive-biases/cognitive-biases/ImplicitAssociationss#Person"/>
        <rdfs:range rdf:resource="https://raw.githubusercontent.com/Maedeam/KRKE-cognitive-biases/modeling-cognitive-biases/cognitive-biases/ImplicitAssociationss#ImplicitAssociationsBias"/>
        <rdfs:comment xml:lang="en">Represents the bias exhibited by individuals toward others based on stereotypical attributes.</rdfs:comment>
        <rdfs:label xml:lang="en">exhibitsBiasTowards</rdfs:label>
    </owl:ObjectProperty>
    


    <!-- https://raw.githubusercontent.com/Maedeam/KRKE-cognitive-biases/modeling-cognitive-biases/cognitive-biases/ImplicitAssociationss#hasAttribute -->

    <owl:ObjectProperty rdf:about="https://raw.githubusercontent.com/Maedeam/KRKE-cognitive-biases/modeling-cognitive-biases/cognitive-biases/ImplicitAssociationss#hasAttribute">
        <rdfs:domain rdf:resource="https://raw.githubusercontent.com/Maedeam/KRKE-cognitive-biases/modeling-cognitive-biases/cognitive-biases/ImplicitAssociationss#Person"/>
        <rdfs:range rdf:resource="https://raw.githubusercontent.com/Maedeam/KRKE-cognitive-biases/modeling-cognitive-biases/cognitive-biases/ImplicitAssociationss#Attribute"/>
        <rdfs:comment xml:lang="en">Relates a person to an attribute that is subject to stereotyping.</rdfs:comment>
        <rdfs:label xml:lang="en">hasAttribute</rdfs:label>
    </owl:ObjectProperty>
    


    <!-- https://raw.githubusercontent.com/Maedeam/KRKE-cognitive-biases/modeling-cognitive-biases/cognitive-biases/ImplicitAssociationss#hasContext -->

    <owl:ObjectProperty rdf:about="https://raw.githubusercontent.com/Maedeam/KRKE-cognitive-biases/modeling-cognitive-biases/cognitive-biases/ImplicitAssociationss#hasContext">
        <rdfs:domain rdf:resource="https://raw.githubusercontent.com/Maedeam/KRKE-cognitive-biases/modeling-cognitive-biases/cognitive-biases/ImplicitAssociationss#ImplicitAssociationsBias"/>
        <rdfs:range rdf:resource="https://raw.githubusercontent.com/Maedeam/KRKE-cognitive-biases/modeling-cognitive-biases/cognitive-biases/ImplicitAssociationss#SocialContext"/>
        <rdfs:comment xml:lang="en">Specifies the context in which Implicit Associations Bias occurs.</rdfs:comment>
        <rdfs:label xml:lang="en">hasContext</rdfs:label>
    </owl:ObjectProperty>
    


    <!-- https://raw.githubusercontent.com/Maedeam/KRKE-cognitive-biases/modeling-cognitive-biases/cognitive-biases/ImplicitAssociationss#hasRelation -->

    <owl:ObjectProperty rdf:about="https://raw.githubusercontent.com/Maedeam/KRKE-cognitive-biases/modeling-cognitive-biases/cognitive-biases/ImplicitAssociationss#hasRelation">
        <rdfs:domain rdf:resource="https://raw.githubusercontent.com/Maedeam/KRKE-cognitive-biases/modeling-cognitive-biases/cognitive-biases/ImplicitAssociationss#ImplicitAssociationsBias"/>
        <rdfs:range rdf:resource="https://raw.githubusercontent.com/Maedeam/KRKE-cognitive-biases/modeling-cognitive-biases/cognitive-biases/ImplicitAssociationss#Attribute"/>
        <rdfs:comment xml:lang="en">Specifies the relation between Implicit Associations Bias and attributes.</rdfs:comment>
        <rdfs:label xml:lang="en">hasRelation</rdfs:label>
    </owl:ObjectProperty>
    


    <!-- https://raw.githubusercontent.com/Maedeam/KRKE-cognitive-biases/modeling-cognitive-biases/cognitive-biases/ImplicitAssociationss#isAffectedBy -->

    <owl:ObjectProperty rdf:about="https://raw.githubusercontent.com/Maedeam/KRKE-cognitive-biases/modeling-cognitive-biases/cognitive-biases/ImplicitAssociationss#isAffectedBy">
        <rdfs:domain rdf:resource="https://raw.githubusercontent.com/Maedeam/KRKE-cognitive-biases/modeling-cognitive-biases/cognitive-biases/ImplicitAssociationss#ImplicitAssociationsBias"/>
        <rdfs:range rdf:resource="https://raw.githubusercontent.com/Maedeam/KRKE-cognitive-biases/modeling-cognitive-biases/cognitive-biases/ImplicitAssociationss#SocialContext"/>
        <rdfs:comment xml:lang="en">Represents the influence of social context on Implicit Associations Bias.</rdfs:comment>
        <rdfs:label xml:lang="en">isAffectedBy</rdfs:label>
    </owl:ObjectProperty>
    


    <!-- 
    ///////////////////////////////////////////////////////////////////////////////////////
    //
    // Classes
    //
    ///////////////////////////////////////////////////////////////////////////////////////
     -->

    


    <!-- https://raw.githubusercontent.com/Maedeam/KRKE-cognitive-biases/modeling-cognitive-biases/cognitive-biases/ImplicitAssociationss#Attribute -->

    <owl:Class rdf:about="https://raw.githubusercontent.com/Maedeam/KRKE-cognitive-biases/modeling-cognitive-biases/cognitive-biases/ImplicitAssociationss#Attribute">
        <rdfs:comment xml:lang="en">Represents characteristics or traits that are subject to stereotyping.</rdfs:comment>
        <rdfs:label xml:lang="en">Attribute</rdfs:label>
    </owl:Class>
    


    <!-- https://raw.githubusercontent.com/Maedeam/KRKE-cognitive-biases/modeling-cognitive-biases/cognitive-biases/ImplicitAssociationss#ChallengeAction -->

    <owl:Class rdf:about="https://raw.githubusercontent.com/Maedeam/KRKE-cognitive-biases/modeling-cognitive-biases/cognitive-biases/ImplicitAssociationss#ChallengeAction">
        <rdfs:comment xml:lang="en">Represents actions or behaviors that challenge or confront Implicit Associations Bias.</rdfs:comment>
        <rdfs:label xml:lang="en">ChallengeAction</rdfs:label>
    </owl:Class>
    


    <!-- https://raw.githubusercontent.com/Maedeam/KRKE-cognitive-biases/modeling-cognitive-biases/cognitive-biases/ImplicitAssociationss#Differentiation -->

    <owl:Class rdf:about="https://raw.githubusercontent.com/Maedeam/KRKE-cognitive-biases/modeling-cognitive-biases/cognitive-biases/ImplicitAssociationss#Differentiation">
        <rdfs:subClassOf rdf:resource="https://raw.githubusercontent.com/Maedeam/KRKE-cognitive-biases/modeling-cognitive-biases/cognitive-biases/ImplicitAssociationss#SocialContext"/>
        <rdfs:comment xml:lang="en">Represents the process of distinguishing or categorizing individuals based on attributes.</rdfs:comment>
        <rdfs:label xml:lang="en">Differentiation</rdfs:label>
    </owl:Class>
    


    <!-- https://raw.githubusercontent.com/Maedeam/KRKE-cognitive-biases/modeling-cognitive-biases/cognitive-biases/ImplicitAssociationss#Gender -->

    <owl:Class rdf:about="https://raw.githubusercontent.com/Maedeam/KRKE-cognitive-biases/modeling-cognitive-biases/cognitive-biases/ImplicitAssociationss#Gender">
        <rdfs:subClassOf rdf:resource="https://raw.githubusercontent.com/Maedeam/KRKE-cognitive-biases/modeling-cognitive-biases/cognitive-biases/ImplicitAssociationss#Attribute"/>
        <rdfs:comment xml:lang="en">Subclass of Attribute, representing gender-related stereotypes.</rdfs:comment>
        <rdfs:label xml:lang="en">Gender</rdfs:label>
    </owl:Class>
    


    <!-- https://raw.githubusercontent.com/Maedeam/KRKE-cognitive-biases/modeling-cognitive-biases/cognitive-biases/ImplicitAssociationss#ImplicitAssociationsBias -->

    <owl:Class rdf:about="https://raw.githubusercontent.com/Maedeam/KRKE-cognitive-biases/modeling-cognitive-biases/cognitive-biases/ImplicitAssociationss#ImplicitAssociationsBias">
        <rdfs:label xml:lang="en">ImplicitAssociationsBias</rdfs:label>
    </owl:Class>
    


    <!-- https://raw.githubusercontent.com/Maedeam/KRKE-cognitive-biases/modeling-cognitive-biases/cognitive-biases/ImplicitAssociationss#Person -->

    <owl:Class rdf:about="https://raw.githubusercontent.com/Maedeam/KRKE-cognitive-biases/modeling-cognitive-biases/cognitive-biases/ImplicitAssociationss#Person">
        <rdfs:label xml:lang="en">Person</rdfs:label>
    </owl:Class>
    


    <!-- https://raw.githubusercontent.com/Maedeam/KRKE-cognitive-biases/modeling-cognitive-biases/cognitive-biases/ImplicitAssociationss#Race -->

    <owl:Class rdf:about="https://raw.githubusercontent.com/Maedeam/KRKE-cognitive-biases/modeling-cognitive-biases/cognitive-biases/ImplicitAssociationss#Race">
        <rdfs:subClassOf rdf:resource="https://raw.githubusercontent.com/Maedeam/KRKE-cognitive-biases/modeling-cognitive-biases/cognitive-biases/ImplicitAssociationss#Attribute"/>
        <rdfs:comment xml:lang="en">Subclass of Attribute, representing racial stereotypes.</rdfs:comment>
        <rdfs:label xml:lang="en">Race</rdfs:label>
    </owl:Class>
    


    <!-- https://raw.githubusercontent.com/Maedeam/KRKE-cognitive-biases/modeling-cognitive-biases/cognitive-biases/ImplicitAssociationss#SocialContext -->

    <owl:Class rdf:about="https://raw.githubusercontent.com/Maedeam/KRKE-cognitive-biases/modeling-cognitive-biases/cognitive-biases/ImplicitAssociationss#SocialContext">
        <rdfs:subClassOf rdf:resource="https://raw.githubusercontent.com/Maedeam/KRKE-cognitive-biases/modeling-cognitive-biases/cognitive-biases/ImplicitAssociationss#ChallengeAction"/>
        <rdfs:comment xml:lang="en">Represents the broader societal or cultural context influencing Implicit Associations Bias.</rdfs:comment>
        <rdfs:label xml:lang="en">SocialContext</rdfs:label>
    </owl:Class>
    


    <!-- 
    ///////////////////////////////////////////////////////////////////////////////////////
    //
    // Individuals
    //
    ///////////////////////////////////////////////////////////////////////////////////////
     -->

    


    <!-- https://raw.githubusercontent.com/Maedeam/KRKE-cognitive-biases/modeling-cognitive-biases/cognitive-biases/ImplicitAssociationss#ChallengeEvent -->

    <owl:NamedIndividual rdf:about="https://raw.githubusercontent.com/Maedeam/KRKE-cognitive-biases/modeling-cognitive-biases/cognitive-biases/ImplicitAssociationss#ChallengeEvent">
        <rdf:type rdf:resource="https://raw.githubusercontent.com/Maedeam/KRKE-cognitive-biases/modeling-cognitive-biases/cognitive-biases/ImplicitAssociationss#ChallengeAction"/>
        <rdfs:comment xml:lang="en">An instance representing a specific event challenging Implicit Associations Bias.</rdfs:comment>
        <rdfs:label xml:lang="en">ChallengeEvent</rdfs:label>
    </owl:NamedIndividual>
    


    <!-- https://raw.githubusercontent.com/Maedeam/KRKE-cognitive-biases/modeling-cognitive-biases/cognitive-biases/ImplicitAssociationss#FashionableAttribute -->

    <owl:NamedIndividual rdf:about="https://raw.githubusercontent.com/Maedeam/KRKE-cognitive-biases/modeling-cognitive-biases/cognitive-biases/ImplicitAssociationss#FashionableAttribute">
        <rdfs:comment xml:lang="en">An attribute related to fashion choices.</rdfs:comment>
        <rdfs:label xml:lang="en">FashionableAttribute</rdfs:label>
    </owl:NamedIndividual>
    


    <!-- https://raw.githubusercontent.com/Maedeam/KRKE-cognitive-biases/modeling-cognitive-biases/cognitive-biases/ImplicitAssociationss#GenderBiasExample -->

    <owl:NamedIndividual rdf:about="https://raw.githubusercontent.com/Maedeam/KRKE-cognitive-biases/modeling-cognitive-biases/cognitive-biases/ImplicitAssociationss#GenderBiasExample">
        <rdf:type rdf:resource="https://raw.githubusercontent.com/Maedeam/KRKE-cognitive-biases/modeling-cognitive-biases/cognitive-biases/ImplicitAssociationss#ImplicitAssociationsBias"/>
        <rdfs:comment xml:lang="en">An instance representing a specific case of gender-based Implicit Associations Bias.</rdfs:comment>
        <rdfs:label xml:lang="en">GenderBiasExample</rdfs:label>
    </owl:NamedIndividual>
    


    <!-- https://raw.githubusercontent.com/Maedeam/KRKE-cognitive-biases/modeling-cognitive-biases/cognitive-biases/ImplicitAssociationss#John -->

    <owl:NamedIndividual rdf:about="https://raw.githubusercontent.com/Maedeam/KRKE-cognitive-biases/modeling-cognitive-biases/cognitive-biases/ImplicitAssociationss#John">
        <rdf:type rdf:resource="https://raw.githubusercontent.com/Maedeam/KRKE-cognitive-biases/modeling-cognitive-biases/cognitive-biases/ImplicitAssociationss#Person"/>
        <rdfs:comment xml:lang="en">An individual person.</rdfs:comment>
        <rdfs:label xml:lang="en">John</rdfs:label>
        <cognitive-biases:ImplicitAssociationsBias.challengesBias rdf:resource="https://raw.githubusercontent.com/Maedeam/KRKE-cognitive-biases/modeling-cognitive-biases/cognitive-biases/ImplicitAssociationss#ChallengeEvent"/>
        <cognitive-biases:ImplicitAssociationsBias.exhibitsBiasTowards rdf:resource="https://raw.githubusercontent.com/Maedeam/KRKE-cognitive-biases/modeling-cognitive-biases/cognitive-biases/ImplicitAssociationss#GenderBiasExample"/>
        <cognitive-biases:ImplicitAssociationsBias.hasAttribute rdf:resource="https://raw.githubusercontent.com/Maedeam/KRKE-cognitive-biases/modeling-cognitive-biases/cognitive-biases/ImplicitAssociationss#FashionableAttribute"/>
    </owl:NamedIndividual>
</rdf:RDF>



<!-- Generated by the OWL API (version 4.5.26.2023-07-17T20:34:13Z) https://github.com/owlcs/owlapi -->

