<?xml version="1.0"?>
<rdf:RDF xmlns="http://www.semanticweb.org/delayed/cognitive-bias-ontology/Negativitybias#"
     xml:base="http://www.semanticweb.org/delayed/cognitive-bias-ontology/Negativitybias"
     xmlns:ns="http://creativecommons.org/ns#"
     xmlns:ns1="http://www.w3.org/2003/06/sw-vocab-status/ns#"
     xmlns:owl="http://www.w3.org/2002/07/owl#"
     xmlns:rdf="http://www.w3.org/1999/02/22-rdf-syntax-ns#"
     xmlns:xml="http://www.w3.org/XML/1998/namespace"
     xmlns:xsd="http://www.w3.org/2001/XMLSchema#"
     xmlns:rdfs="http://www.w3.org/2000/01/rdf-schema#"
     xmlns:vann="http://purl.org/vocab/vann/"
     xmlns:terms="http://purl.org/dc/terms/"
     xmlns:HaloEffect="https://raw.githubusercontent.com/Maedeam/KRKE-cognitive-biases/modeling-cognitive-biases/cognitive-biases/Negativitybias.owl"
     xmlns:HaloEffect1="https://raw.githubusercontent.com/Maedeam/KRKE-cognitive-biases/modeling-cognitive-biases/cognitive-biases/Negativitybias.owl#"
     xmlns:description="http://www.ontologydesignpatterns.org/cp/owl/description.owl#"
     xmlns:cpannotationschema="http://www.ontologydesignpatterns.org/schemas/cpannotationschema.owl#">
    <owl:Ontology rdf:about="https://raw.githubusercontent.com/Maedeam/KRKE-cognitive-biases/modeling-cognitive-biases/cognitive-biases/Negativitybias.owl">
        <owl:versionIRI rdf:resource="https://raw.githubusercontent.com/Maedeam/KRKE-cognitive-biases/modeling-cognitive-biases/cognitive-biases/Negativitybias.owl"/>
        <terms:creator xml:lang="en">Atousa Heidarnia</terms:creator>
        <terms:creator xml:lang="en">Maede Hajjari</terms:creator>
        <terms:description xml:lang="en">Negativity bias module of the Cognitive Bias Ontology.</terms:description>
        <terms:hasVersion xml:lang="en">0.1</terms:hasVersion>
        <terms:title xml:lang="en">Negativity bias Ontology</terms:title>
        <rdfs:comment xml:lang="en">The &quot;Negativity bias&quot; is the psychological tendency to give more weight and attention to negative information or experiences than positive ones.</rdfs:comment>
    </owl:Ontology>
    


    <!-- 
    ///////////////////////////////////////////////////////////////////////////////////////
    //
    // Object Properties
    //
    ///////////////////////////////////////////////////////////////////////////////////////
     -->


    <owl:ObjectProperty rdf:about="http://www.ontologydesignpatterns.org/cp/owl/description.owl#influences">
        <rdfs:domain rdf:resource="https://w3id.org/framester/data/framestercore/PerceptionExperience"/>
        <rdfs:range rdf:resource="https://w3id.org/framester/data/framestercore/Awareness"/>
        <rdfs:comment>Describes the relationship between the UserPerceptionAnalysis class and the cognitive processes it influences, such as the DecisionMakingProcess.</rdfs:comment>
        <rdfs:label>influences</rdfs:label>
    </owl:ObjectProperty>
    


    <owl:ObjectProperty rdf:about="http://www.ontologydesignpatterns.org/cp/owl/description.owl#focusesOn">
        <rdfs:domain rdf:resource="https://w3id.org/framester/data/framestercore/PerceptionExperience"/>
        <rdfs:range rdf:resource="https://w3id.org/framester/data/framestercore/Obviousness"/>
        <rdfs:comment>Describes the relationship between the UserPerceptionAnalysis class and the specific focus on information, such as Fixation on negative aspects.</rdfs:comment>
        <rdfs:label>focusesOn</rdfs:label>
    </owl:ObjectProperty>
    


    <owl:ObjectProperty rdf:about="http://www.ontologydesignpatterns.org/cp/owl/description.owl#providesReview">
        <rdfs:domain rdf:resource="https://w3id.org/framester/data/framestercore/Inspecting"/>
        <rdfs:comment>Describes the relationship between the ReviewerRole class and the specific reviews they provide, which may include AdverseEvaluations.</rdfs:comment>
        <rdfs:label>providesReview</rdfs:label>
    </owl:ObjectProperty>


    <owl:ObjectProperty rdf:about="http://www.ontologydesignpatterns.org/cp/owl/description.owl#experiencedEmotion">
        <rdfs:domain rdf:resource="https://w3id.org/framester/data/framestercore/Response"/>
        <rdfs:range rdf:resource="https://w3id.org/framester/data/framestercore/EmotionDirected"/>
        <rdfs:comment>Describes the relationship between the EmotionalResponse class and the specific emotional distress individuals may experience.</rdfs:comment>
        <rdfs:label>experiencedEmotion</rdfs:label>
    </owl:ObjectProperty>
    


    <!-- 
    ///////////////////////////////////////////////////////////////////////////////////////
    //
    // Classes
    //
    ///////////////////////////////////////////////////////////////////////////////////////
     -->

    

    <owl:Class rdf:about="https://w3id.org/framester/data/framestercore/EmotionDirected">
        <rdfs:subClassOf rdf:resource="https://w3id.org/framester/data/framestercore/PerceptionExperience"/>
        <rdfs:comment>A subclass of EmotionalResponse that specifically denotes heightened emotional responses, such as DisproportionateDistress.</rdfs:comment>
        <rdfs:label>EmotionalDistress</rdfs:label>
    </owl:Class>
    

    <owl:Class rdf:about="https://w3id.org/framester/data/framestercore/Response">
        <rdfs:subClassOf rdf:resource="https://w3id.org/framester/data/framestercore/PerceptionExperience"/>
        <rdfs:comment>A subclass of UserPerceptionAnalysis representing emotional reactions individuals may experience, including heightened emotional responses influenced by the Negativity Bias.</rdfs:comment>
        <rdfs:label>EmotionalResponse</rdfs:label>
    </owl:Class>
    


    <owl:Class rdf:about="https://w3id.org/framester/data/framestercore/Obviousness">
        <rdfs:subClassOf rdf:resource="https://w3id.org/framester/data/framestercore/PerceptionExperience"/>
        <rdfs:comment>A subclass of UserPerceptionAnalysis representing the selective attention individuals exhibit, as seen in Fixation on specific information.</rdfs:comment>
        <rdfs:label>InformationFocus</rdfs:label>
    </owl:Class>
    


    <owl:Class rdf:about="https://w3id.org/framester/data/framestercore/Inspecting">
        <rdfs:subClassOf rdf:resource="https://w3id.org/framester/data/framestercore/PerceptionExperience"/>
        <rdfs:comment>A subclass of UserPerceptionAnalysis representing the role of individuals who provide reviews, influencing the ReviewAnalysis process.</rdfs:comment>
        <rdfs:label>ReviewerRole</rdfs:label>
    </owl:Class>
    


    <owl:Class rdf:about="https://w3id.org/framester/data/framestercore/Deciding">
        <rdfs:subClassOf rdf:resource="https://w3id.org/framester/data/framestercore/Awareness"/>
        <rdfs:comment>A subclass of CognitiveProcesses representing the cognitive steps individuals take when making choices, influenced by factors including the Negativity Bias.</rdfs:comment>
        <rdfs:label>DecisionMakingProcess</rdfs:label>
    </owl:Class>
    



    <owl:Class rdf:about="https://w3id.org/framester/data/framestercore/Awareness">
        <rdfs:subClassOf rdf:resource="https://w3id.org/framester/data/framestercore/PerceptionExperience"/>
        <rdfs:comment>A subclass of UserPerceptionAnalysis that focuses on mental processes involved in information perception and processing.</rdfs:comment>
        <rdfs:label>CognitiveProcesses</rdfs:label>
    </owl:Class>
    

    <owl:Class rdf:about="https://w3id.org/framester/data/framestercore/Assessing">
        <rdfs:subClassOf rdf:resource="https://w3id.org/framester/data/framestercore/PerceptionExperience"/>
        <rdfs:comment>A subclass of UserPerceptionAnalysis representing the examination of reviews, including AdverseEvaluation, as part of the cognitive processes influenced by the Negativity Bias.</rdfs:comment>
        <rdfs:label>ReviewAnalysis</rdfs:label>
    </owl:Class>
    

    <owl:Class rdf:about="https://w3id.org/framester/data/framestercore/PerceptionExperience">
        <rdfs:comment>The overarching class representing the analysis of user perception, encompassing various factors such as cognitive processes, emotional responses, and review analysis.</rdfs:comment>
        <rdfs:label>UserPerceptionAnalysis</rdfs:label>
    </owl:Class>
    


    <owl:Class rdf:about="https://w3id.org/framester/data/framestercore/Examination">
        <rdfs:subClassOf rdf:resource="https://w3id.org/framester/data/framestercore/PerceptionExperience"/>
        <rdfs:comment>representing a review or evaluation that emphasizes negative aspects of a subject, serving as a stimulus for the activation of the Negativity Bias.</rdfs:comment>
        <rdfs:label>AdverseEvaluation</rdfs:label>
    </owl:Class>
    


    <!-- 
    ///////////////////////////////////////////////////////////////////////////////////////
    //
    // Individuals
    //
    ///////////////////////////////////////////////////////////////////////////////////////
     -->



    <owl:NamedIndividual rdf:about="https://w3id.org/framester/data/framestercore/People">
        <rdfs:comment>An individual representing the role of a person who contributes reviews, influencing the overall review analysis and potentially contributing to the activation of the Negativity Bias.</rdfs:comment>
        <rdfs:label>Reviewer</rdfs:label>
    </owl:NamedIndividual>
</rdf:RDF>



<!-- Generated by the OWL API (version 4.5.13) https://github.com/owlcs/owlapi -->
