<?xml version="1.0"?>
<rdf:RDF xmlns="http://www.semanticweb.org/delayed/cognitive-bias-ontology/Prejudice#"
     xml:base="http://www.semanticweb.org/delayed/cognitive-bias-ontology/Prejudice"
     xmlns:ns="http://creativecommons.org/ns#"
     xmlns:ns1="http://www.w3.org/2003/06/sw-vocab-status/ns#"
     xmlns:owl="http://www.w3.org/2002/07/owl#"
     xmlns:rdf="http://www.w3.org/1999/02/22-rdf-syntax-ns#"
     xmlns:xml="http://www.w3.org/XML/1998/namespace"
     xmlns:xsd="http://www.w3.org/2001/XMLSchema#"
     xmlns:rdfs="http://www.w3.org/2000/01/rdf-schema#"
     xmlns:vann="http://purl.org/vocab/vann/"
     xmlns:terms="http://purl.org/dc/terms/"
     xmlns:HaloEffect="https://raw.githubusercontent.com/Maedeam/KRKE-cognitive-biases/modeling-cognitive-biases/cognitive-biases/Prejudice.owl"
     xmlns:HaloEffect1="https://raw.githubusercontent.com/Maedeam/KRKE-cognitive-biases/modeling-cognitive-biases/cognitive-biases/Prejudice.owl#"
     xmlns:description="http://www.ontologydesignpatterns.org/cp/owl/description.owl#"
     xmlns:cpannotationschema="http://www.ontologydesignpatterns.org/schemas/cpannotationschema.owl#">
    <owl:Ontology rdf:about="https://raw.githubusercontent.com/Maedeam/KRKE-cognitive-biases/modeling-cognitive-biases/cognitive-biases/Prejudice.owl">
        <owl:versionIRI rdf:resource="https://raw.githubusercontent.com/Maedeam/KRKE-cognitive-biases/modeling-cognitive-biases/cognitive-biases/Prejudice.owl"/>
        <terms:creator xml:lang="en">Atousa Heidarnia</terms:creator>
        <terms:creator xml:lang="en">Maede Hajjari</terms:creator>
        <terms:description xml:lang="en">Prejudice module of the Cognitive Bias Ontology.</terms:description>
        <terms:hasVersion xml:lang="en">0.1</terms:hasVersion>
        <terms:title xml:lang="en">Prejudice Ontology</terms:title>
        <rdfs:comment xml:lang="en">The &quot;Prejudice&quot;is a preconceived opinion or feeling, usually unfavorable, formed without knowledge, reason, or actual experience.</rdfs:comment>
    </owl:Ontology>
    

    <!-- 
    ///////////////////////////////////////////////////////////////////////////////////////
    //
    // Object Properties
    //
    ///////////////////////////////////////////////////////////////////////////////////////
     -->

    


   

    <owl:ObjectProperty rdf:about="http://www.ontologydesignpatterns.org/cp/owl/description.owl#involvesAgent">
        <rdfs:domain rdf:resource="https://w3id.org/framester/data/framestercore/Quantity"/>
        <rdfs:domain rdf:resource="https://w3id.org/framester/data/framestercore/Process"/>
        <rdfs:domain rdf:resource="https://w3id.org/framester/data/framestercore/Differentiation"/>
        <rdfs:range rdf:resource="https://w3id.org/framester/data/framestercore/People"/>
        <rdfs:label>involvesAgent</rdfs:label>
    </owl:ObjectProperty>
    


    <owl:ObjectProperty rdf:about="http://www.ontologydesignpatterns.org/cp/owl/description.owl#manifestsIn">
        <rdfs:domain rdf:resource="https://w3id.org/framester/data/framestercore/Partiality"/>
        <rdfs:range rdf:resource="https://w3id.org/framester/data/framestercore/StateOfEntity"/>
        <rdfs:comment>Indicates the situations or contexts in which prejudice becomes evident.</rdfs:comment>
        <rdfs:label>manifestsIn</rdfs:label>
    </owl:ObjectProperty>
    


    <owl:ObjectProperty rdf:about="http://www.ontologydesignpatterns.org/cp/owl/description.owl#occursIn">
        <rdfs:domain rdf:resource="https://w3id.org/framester/data/framestercore/Quantity"/>
        <rdfs:domain rdf:resource="https://w3id.org/framester/data/framestercore/Differentiation"/>
        <rdfs:domain rdf:resource="https://w3id.org/framester/data/framestercore/Process"/>
        <rdfs:range rdf:resource="https://w3id.org/framester/data/framestercore/StateOfEntity"/>
        <rdfs:label>occursIn</rdfs:label>
    </owl:ObjectProperty>
    


    <!-- 
    ///////////////////////////////////////////////////////////////////////////////////////
    //
    // Classes
    //
    ///////////////////////////////////////////////////////////////////////////////////////
     -->

    

    <owl:Class rdf:about="https://w3id.org/framester/data/framestercore/Partiality">
        <rdfs:comment>encompassing all forms of preconceived and unjust judgments or opinions</rdfs:comment>
        <rdfs:label>Prejudice</rdfs:label>
    </owl:Class>
    


   
    <owl:Class rdf:about="https://w3id.org/framester/data/framestercore/Process">
        <rdfs:comment>representing instances where individuals or groups are pushed to the sidelines or excluded unfairly.</rdfs:comment>
        <rdfs:label>Marginalization</rdfs:label>
    </owl:Class>
    


    <owl:Class rdf:about="https://w3id.org/framester/data/framestercore/People">
        <rdfs:comment>representing individuals or entities involved in the perpetuation or experience of prejudice.</rdfs:comment>
        <rdfs:label>Agent</rdfs:label>
    </owl:Class>
    



    <owl:Class rdf:about="https://w3id.org/framester/data/framestercore/Differentiation">
        <rdfs:comment>focusing on biased treatment or unfair actions against individuals or groups.</rdfs:comment>
        <rdfs:label>Discrimination</rdfs:label>
    </owl:Class>
    


    <owl:Class rdf:about="https://w3id.org/framester/data/framestercore/Quantity">
        <rdfs:comment>highlighting instances where judgments are made based on surface-level attributes rather than meaningful qualities.</rdfs:comment>
        <rdfs:label>Superficiality</rdfs:label>
    </owl:Class>
    

    <owl:Class rdf:about="https://w3id.org/framester/data/framestercore/StateOfEntity">
        <rdfs:comment>representing the context or circumstances in which prejudice manifests</rdfs:comment>
        <rdfs:label>Situation</rdfs:label>
    </owl:Class>
</rdf:RDF>



<!-- Generated by the OWL API (version 4.5.13) https://github.com/owlcs/owlapi -->
