<?xml version="1.0"?>
<rdf:RDF xmlns="http://www.semanticweb.org/delayed/cognitive-bias-ontology/StereotypicalBias#"
     xml:base="http://www.semanticweb.org/delayed/cognitive-bias-ontology/StereotypicalBias"
     xmlns:ns="http://creativecommons.org/ns#"
     xmlns:ns1="http://www.w3.org/2003/06/sw-vocab-status/ns#"
     xmlns:owl="http://www.w3.org/2002/07/owl#"
     xmlns:rdf="http://www.w3.org/1999/02/22-rdf-syntax-ns#"
     xmlns:xml="http://www.w3.org/XML/1998/namespace"
     xmlns:xsd="http://www.w3.org/2001/XMLSchema#"
     xmlns:rdfs="http://www.w3.org/2000/01/rdf-schema#"
     xmlns:skos="http://www.w3.org/2004/02/skos/core#"
     xmlns:vann="http://purl.org/vocab/vann/"
     xmlns:terms="http://purl.org/dc/terms/"
     xmlns:description="http://www.ontologydesignpatterns.org/cp/owl/description.owl#"
     xmlns:StereotypicalBias="https://raw.githubusercontent.com/Maedeam/KRKE-cognitive-biases/modeling-cognitive-biases/cognitive-biases/StereotypicalBias.owl"
     xmlns:StereotypicalBias1="https://raw.githubusercontent.com/Maedeam/KRKE-cognitive-biases/modeling-cognitive-biases/cognitive-biases/StereotypicalBias.owl#"
     xmlns:StereotypicalBias2="https://raw.githubusercontent.com/Maedeam/KRKE-cognitive-biases/modeling-cognitive-biases/cognitive-biases/StereotypicalBias#"
     xmlns:cpannotationschema="http://www.ontologydesignpatterns.org/schemas/cpannotationschema.owl#">
    <owl:Ontology rdf:about="https://raw.githubusercontent.com/Maedeam/KRKE-cognitive-biases/modeling-cognitive-biases/cognitive-biases/StereotypicalBias.owl">
        <owl:versionIRI rdf:resource="https://raw.githubusercontent.com/Maedeam/KRKE-cognitive-biases/modeling-cognitive-biases/cognitive-biases/StereotypicalBias.owl"/>
        <terms:creator xml:lang="en">Atousa Heidarnia</terms:creator>
        <terms:creator xml:lang="en">Maede Hajjari</terms:creator>
        <terms:description xml:lang="en">Stereotypical Bias module of the Cognitive Bias Ontology.</terms:description>
        <terms:hasVersion xml:lang="en">0.1</terms:hasVersion>
        <terms:title xml:lang="en">Stereotypical Bias Ontology</terms:title>
        <rdfs:comment xml:lang="en">Stereotypical bias, also known as stereotyping, refers to the cognitive inclination to generalize and apply predefined characteristics or traits to individuals based on their membership in a particular social group. This bias often stems from preconceived notions, cultural expectations, or widely held beliefs about specific groups, leading individuals to make assumptions about others without considering their unique qualities or individual differences. Stereotypical bias can influence perceptions, decisions, and interactions, contributing to the perpetuation of social stereotypes and potentially resulting in unfair judgments or discriminatory behaviors.</rdfs:comment>
    </owl:Ontology>
    


    <!-- 
    ///////////////////////////////////////////////////////////////////////////////////////
    //
    // Annotation properties
    //
    ///////////////////////////////////////////////////////////////////////////////////////
     -->

    


    <!-- http://purl.org/dc/terms/creator -->

    <owl:AnnotationProperty rdf:about="http://purl.org/dc/terms/creator"/>
    


    <!-- http://purl.org/dc/terms/description -->

    <owl:AnnotationProperty rdf:about="http://purl.org/dc/terms/description"/>
    


    <!-- http://purl.org/dc/terms/hasVersion -->

    <owl:AnnotationProperty rdf:about="http://purl.org/dc/terms/hasVersion"/>
    


    <!-- http://purl.org/dc/terms/title -->

    <owl:AnnotationProperty rdf:about="http://purl.org/dc/terms/title"/>
    


    <!-- http://www.w3.org/2004/02/skos/core#comment -->

    <owl:AnnotationProperty rdf:about="http://www.w3.org/2004/02/skos/core#comment"/>
    


    <!-- 
    ///////////////////////////////////////////////////////////////////////////////////////
    //
    // Object Properties
    //
    ///////////////////////////////////////////////////////////////////////////////////////
     -->

    


    <!-- https://raw.githubusercontent.com/Maedeam/KRKE-cognitive-biases/modeling-cognitive-biases/cognitive-biases/StereotypicalBias#challengesBias -->

    <owl:ObjectProperty rdf:about="https://raw.githubusercontent.com/Maedeam/KRKE-cognitive-biases/modeling-cognitive-biases/cognitive-biases/StereotypicalBias#challengesBias">
        <rdfs:domain rdf:resource="https://raw.githubusercontent.com/Maedeam/KRKE-cognitive-biases/modeling-cognitive-biases/cognitive-biases/StereotypicalBias#Person"/>
        <rdfs:range rdf:resource="https://raw.githubusercontent.com/Maedeam/KRKE-cognitive-biases/modeling-cognitive-biases/cognitive-biases/StereotypicalBias#ChallengeAction"/>
        <rdfs:comment xml:lang="en">Represents actions or behaviors that challenge or confront stereotypical biases.</rdfs:comment>
        <rdfs:label xml:lang="en">challengesBias</rdfs:label>
    </owl:ObjectProperty>
    


    <!-- https://raw.githubusercontent.com/Maedeam/KRKE-cognitive-biases/modeling-cognitive-biases/cognitive-biases/StereotypicalBias#exhibitsBiasTowards -->

    <owl:ObjectProperty rdf:about="https://raw.githubusercontent.com/Maedeam/KRKE-cognitive-biases/modeling-cognitive-biases/cognitive-biases/StereotypicalBias#exhibitsBiasTowards">
        <rdfs:domain rdf:resource="https://raw.githubusercontent.com/Maedeam/KRKE-cognitive-biases/modeling-cognitive-biases/cognitive-biases/StereotypicalBias#Person"/>
        <rdfs:range rdf:resource="https://raw.githubusercontent.com/Maedeam/KRKE-cognitive-biases/modeling-cognitive-biases/cognitive-biases/StereotypicalBias#StereotypicalBias"/>
        <rdfs:comment xml:lang="en">Represents the bias exhibited by individuals toward others based on stereotypical attributes.</rdfs:comment>
        <rdfs:label xml:lang="en">exhibitsBiasTowards</rdfs:label>
    </owl:ObjectProperty>
    


    <!-- https://raw.githubusercontent.com/Maedeam/KRKE-cognitive-biases/modeling-cognitive-biases/cognitive-biases/StereotypicalBias#hasAttribute -->

    <owl:ObjectProperty rdf:about="https://raw.githubusercontent.com/Maedeam/KRKE-cognitive-biases/modeling-cognitive-biases/cognitive-biases/StereotypicalBias#hasAttribute">
        <rdfs:domain rdf:resource="https://raw.githubusercontent.com/Maedeam/KRKE-cognitive-biases/modeling-cognitive-biases/cognitive-biases/StereotypicalBias#Person"/>
        <rdfs:range rdf:resource="https://en.wiktionary.org/wiki/attribute"/>
        <rdfs:comment xml:lang="en">Relates a person to an attribute that is subject to stereotyping.</rdfs:comment>
        <rdfs:label xml:lang="en">hasAttribute</rdfs:label>
    </owl:ObjectProperty>
    


    <!-- https://raw.githubusercontent.com/Maedeam/KRKE-cognitive-biases/modeling-cognitive-biases/cognitive-biases/StereotypicalBias#isAffectedBy -->

    <owl:ObjectProperty rdf:about="https://raw.githubusercontent.com/Maedeam/KRKE-cognitive-biases/modeling-cognitive-biases/cognitive-biases/StereotypicalBias#isAffectedBy">
        <rdfs:domain rdf:resource="https://raw.githubusercontent.com/Maedeam/KRKE-cognitive-biases/modeling-cognitive-biases/cognitive-biases/StereotypicalBias#StereotypicalBias"/>
        <rdfs:range rdf:resource="https://raw.githubusercontent.com/Maedeam/KRKE-cognitive-biases/modeling-cognitive-biases/cognitive-biases/StereotypicalBias#SocialContext"/>
        <rdfs:comment xml:lang="en">Represents the influence of social context on stereotypical biases.</rdfs:comment>
        <rdfs:label xml:lang="en">isAffectedBy</rdfs:label>
    </owl:ObjectProperty>
    


    <!-- 
    ///////////////////////////////////////////////////////////////////////////////////////
    //
    // Classes
    //
    ///////////////////////////////////////////////////////////////////////////////////////
     -->

    


    <!-- http://etna.istc.cnr.it/framester2/data/framestercore/Differentiation -->

    <owl:Class rdf:about="http://etna.istc.cnr.it/framester2/data/framestercore/Differentiation">
        <rdfs:comment xml:lang="en">Represents the process of distinguishing or categorizing individuals based on attributes.</rdfs:comment>
        <rdfs:label xml:lang="en">Differentiation</rdfs:label>
    </owl:Class>
    


    <!-- https://en.wiktionary.org/wiki/attribute -->

    <owl:Class rdf:about="https://en.wiktionary.org/wiki/attribute">
        <rdfs:comment xml:lang="en">Represents characteristics or traits that are subject to stereotyping.</rdfs:comment>
        <rdfs:label xml:lang="en">Attribute</rdfs:label>
    </owl:Class>
    


    <!-- https://raw.githubusercontent.com/Maedeam/KRKE-cognitive-biases/modeling-cognitive-biases/cognitive-biases/StereotypicalBias#ChallengeAction -->

    <owl:Class rdf:about="https://raw.githubusercontent.com/Maedeam/KRKE-cognitive-biases/modeling-cognitive-biases/cognitive-biases/StereotypicalBias#ChallengeAction">
        <rdfs:comment xml:lang="en">Represents actions or behaviors that challenge or confront stereotypical biases.</rdfs:comment>
        <rdfs:label xml:lang="en">ChallengeAction</rdfs:label>
    </owl:Class>
    


    <!-- https://raw.githubusercontent.com/Maedeam/KRKE-cognitive-biases/modeling-cognitive-biases/cognitive-biases/StereotypicalBias#Gender -->

    <owl:Class rdf:about="https://raw.githubusercontent.com/Maedeam/KRKE-cognitive-biases/modeling-cognitive-biases/cognitive-biases/StereotypicalBias#Gender">
        <rdfs:subClassOf rdf:resource="https://en.wiktionary.org/wiki/attribute"/>
        <rdfs:comment xml:lang="en">Subclass of Attribute, representing gender-related stereotypes.</rdfs:comment>
        <rdfs:label xml:lang="en">Gender</rdfs:label>
    </owl:Class>
    


    <!-- https://raw.githubusercontent.com/Maedeam/KRKE-cognitive-biases/modeling-cognitive-biases/cognitive-biases/StereotypicalBias#Person -->

    <owl:Class rdf:about="https://raw.githubusercontent.com/Maedeam/KRKE-cognitive-biases/modeling-cognitive-biases/cognitive-biases/StereotypicalBias#Person">
        <rdfs:comment xml:lang="en">Represents individuals in the context of stereotypical bias.</rdfs:comment>
        <rdfs:label xml:lang="en">Person</rdfs:label>
    </owl:Class>
    


    <!-- https://raw.githubusercontent.com/Maedeam/KRKE-cognitive-biases/modeling-cognitive-biases/cognitive-biases/StereotypicalBias#Race -->

    <owl:Class rdf:about="https://raw.githubusercontent.com/Maedeam/KRKE-cognitive-biases/modeling-cognitive-biases/cognitive-biases/StereotypicalBias#Race">
        <rdfs:subClassOf rdf:resource="https://en.wiktionary.org/wiki/attribute"/>
        <rdfs:comment xml:lang="en">Subclass of Attribute, representing racial stereotypes.</rdfs:comment>
        <rdfs:label xml:lang="en">Race</rdfs:label>
    </owl:Class>
    


    <!-- https://raw.githubusercontent.com/Maedeam/KRKE-cognitive-biases/modeling-cognitive-biases/cognitive-biases/StereotypicalBias#SocialContext -->

    <owl:Class rdf:about="https://raw.githubusercontent.com/Maedeam/KRKE-cognitive-biases/modeling-cognitive-biases/cognitive-biases/StereotypicalBias#SocialContext">
        <rdfs:comment xml:lang="en">Represents the broader societal or cultural context influencing stereotypical biases.</rdfs:comment>
        <rdfs:label xml:lang="en">SocialContext</rdfs:label>
    </owl:Class>
    


    <!-- https://raw.githubusercontent.com/Maedeam/KRKE-cognitive-biases/modeling-cognitive-biases/cognitive-biases/StereotypicalBias#StereotypicalBias -->

    <owl:Class rdf:about="https://raw.githubusercontent.com/Maedeam/KRKE-cognitive-biases/modeling-cognitive-biases/cognitive-biases/StereotypicalBias#StereotypicalBias">
        <rdfs:comment xml:lang="en">Represents the overarching concept of stereotypical bias.</rdfs:comment>
        <rdfs:label xml:lang="en">StereotypicalBias</rdfs:label>
    </owl:Class>
    


    <!-- 
    ///////////////////////////////////////////////////////////////////////////////////////
    //
    // Individuals
    //
    ///////////////////////////////////////////////////////////////////////////////////////
     -->

    


    <!-- https://raw.githubusercontent.com/Maedeam/KRKE-cognitive-biases/modeling-cognitive-biases/cognitive-biases/StereotypicalBias#ChallengeEvent -->

    <owl:NamedIndividual rdf:about="https://raw.githubusercontent.com/Maedeam/KRKE-cognitive-biases/modeling-cognitive-biases/cognitive-biases/StereotypicalBias#ChallengeEvent">
        <rdf:type rdf:resource="https://raw.githubusercontent.com/Maedeam/KRKE-cognitive-biases/modeling-cognitive-biases/cognitive-biases/StereotypicalBias#ChallengeAction"/>
        <rdfs:comment xml:lang="en">An instance representing a specific event challenging stereotypical biases.</rdfs:comment>
        <rdfs:label xml:lang="en">ChallengeEvent</rdfs:label>
    </owl:NamedIndividual>
    


    <!-- https://raw.githubusercontent.com/Maedeam/KRKE-cognitive-biases/modeling-cognitive-biases/cognitive-biases/StereotypicalBias#FashionableAttribute -->

    <owl:NamedIndividual rdf:about="https://raw.githubusercontent.com/Maedeam/KRKE-cognitive-biases/modeling-cognitive-biases/cognitive-biases/StereotypicalBias#FashionableAttribute">
        <rdf:type rdf:resource="https://en.wiktionary.org/wiki/attribute"/>
        <rdfs:comment xml:lang="en">An attribute related to fashion choices.</rdfs:comment>
        <rdfs:label xml:lang="en">FashionableAttribute</rdfs:label>
    </owl:NamedIndividual>
    


    <!-- https://raw.githubusercontent.com/Maedeam/KRKE-cognitive-biases/modeling-cognitive-biases/cognitive-biases/StereotypicalBias#GenderBiasExample -->

    <owl:NamedIndividual rdf:about="https://raw.githubusercontent.com/Maedeam/KRKE-cognitive-biases/modeling-cognitive-biases/cognitive-biases/StereotypicalBias#GenderBiasExample">
        <rdf:type rdf:resource="https://raw.githubusercontent.com/Maedeam/KRKE-cognitive-biases/modeling-cognitive-biases/cognitive-biases/StereotypicalBias#StereotypicalBias"/>
        <rdfs:comment xml:lang="en">An instance representing a specific case of gender-based stereotypical bias.</rdfs:comment>
        <rdfs:label xml:lang="en">GenderBiasExample</rdfs:label>
    </owl:NamedIndividual>
    


    <!-- https://raw.githubusercontent.com/Maedeam/KRKE-cognitive-biases/modeling-cognitive-biases/cognitive-biases/StereotypicalBias#John -->

    <owl:NamedIndividual rdf:about="https://raw.githubusercontent.com/Maedeam/KRKE-cognitive-biases/modeling-cognitive-biases/cognitive-biases/StereotypicalBias#John">
        <rdf:type rdf:resource="https://raw.githubusercontent.com/Maedeam/KRKE-cognitive-biases/modeling-cognitive-biases/cognitive-biases/StereotypicalBias#Person"/>
        <StereotypicalBias2:challengesBias rdf:resource="https://raw.githubusercontent.com/Maedeam/KRKE-cognitive-biases/modeling-cognitive-biases/cognitive-biases/StereotypicalBias#ChallengeEvent"/>
        <StereotypicalBias2:exhibitsBiasTowards rdf:resource="https://raw.githubusercontent.com/Maedeam/KRKE-cognitive-biases/modeling-cognitive-biases/cognitive-biases/StereotypicalBias#GenderBiasExample"/>
        <StereotypicalBias2:hasAttribute rdf:resource="https://raw.githubusercontent.com/Maedeam/KRKE-cognitive-biases/modeling-cognitive-biases/cognitive-biases/StereotypicalBias#FashionableAttribute"/>
        <rdfs:comment xml:lang="en">An individual person.</rdfs:comment>
        <rdfs:label xml:lang="en">John</rdfs:label>
    </owl:NamedIndividual>
</rdf:RDF>



<!-- Generated by the OWL API (version 4.5.26.2023-07-17T20:34:13Z) https://github.com/owlcs/owlapi -->

